smc/SMC.ec
@@ -1,6 +1,6 @@
 (* SMC.ec *)
 
-prover ["!"].  (* no provers *)
+prover quorum=2 ["Alt-Ergo" "Z3"].
 
 require import AllCore List FSet Distr ListPO.
 require DDH UCCore.
@@ -103,18 +103,18 @@ op gen_rel (x : bits) (q : exp) : bool = x = g ^ q.
 
 op log (x : bits) : exp = choiceb (gen_rel x) e.
 
-lemma log_gen (q : exp) : log (gen q) = q.
+lemma log_genK : cancel gen log.
 proof.
-rewrite /gen /log.
+rewrite /gen /log /cancel => q.
 have choice_g2q := choicebP (gen_rel (g ^ q)) e.
 have /choice_g2q @/gen_rel /gen_inj {2}-> // :
   exists (q' : exp), gen_rel (g ^ q) q'
   by rewrite /gen_rel; by exists q.
 qed.
 
-lemma gen_log (x : bits) : gen (log x) = x.
+lemma gen_logK : cancel log gen.
 proof.
-rewrite /gen /log.
+rewrite /gen /log /cancel => x.
 have @/gen_rel <- // := choicebP (gen_rel x) e.
 rewrite gen_surj.
 qed.
@@ -206,7 +206,7 @@ op dec_fw_req (m : msg) : (addr * port * port * univ) option =
         let (v1, v2) = oget (dec_univ_pair v)
         in (! is_univ_port v1) ?
            None :
-           Some (pt1.`1, pt2, oget(dec_univ_port v1), v2).
+           Some (pt1.`1, pt2, oget (dec_univ_port v1), v2).
 
 lemma enc_dec_fw_req (func : addr, pt1 pt2 : port, u : univ) :
   dec_fw_req (fw_req func pt1 pt2 u) = Some (func, pt1, pt2, u).
@@ -232,7 +232,7 @@ op dec_fw_rsp (m : msg) : (addr * port * port * univ) option =
         let (v1, v2) = oget (dec_univ_pair v)
         in (! is_univ_port v1) ?
            None :
-           Some (pt2.`1, oget(dec_univ_port v1), pt1, v2).
+           Some (pt2.`1, oget (dec_univ_port v1), pt1, v2).
 
 lemma enc_dec_fw_rsp (func : addr, pt1 pt2 : port, u : univ) :
   dec_fw_rsp (fw_rsp func pt1 pt2 u) = Some (func, pt1, pt2, u).
@@ -262,8 +262,8 @@ op dec_fw_obs (m : msg) : (addr * addr * port * port * univ) option =
         in (! is_univ_port v1 \/ ! is_univ_port v2) ?
            None :
            Some (pt2.`1, pt1.`1,
-                 oget(dec_univ_port v1),
-                 oget(dec_univ_port v2),
+                 oget (dec_univ_port v1),
+                 oget (dec_univ_port v2),
                  v3).
 
 lemma enc_dec_fw_obs (func adv : addr, pt1 pt2 : port, u : univ) :
@@ -305,14 +305,14 @@ proof. done. qed.
 
 type fw_state = [
     FwStateInit
-  | FwStateWait of (port * port * univ)
-  | FwStateFinal
+  | FwStateWait  of (port * port * univ)
+  | FwStateFinal of (port * port * univ)
 ].
 
 op dec_fw_state_wait (st : fw_state) : (port * port * univ) option =
-     with st = FwStateInit   => None
-     with st = FwStateWait t => Some t
-     with st = FwStateFinal  => None.
+     with st = FwStateInit    => None
+     with st = FwStateWait t  => Some t
+     with st = FwStateFinal _ => None.
 
 lemma enc_dec_fw_state_wait (t : port * port * univ) :
   dec_fw_state_wait (FwStateWait t) = Some t.
@@ -323,6 +323,22 @@ op is_fw_state_wait (st : fw_state) : bool =
 
 lemma is_fw_state_wait (t : port * port * univ) :
   is_fw_state_wait (FwStateWait t).
+proof. done. qed.
+
+op dec_fw_state_final (st : fw_state) : (port * port * univ) option =
+     with st = FwStateInit    => None
+     with st = FwStateWait _  => None
+     with st = FwStateFinal x => Some x.
+
+lemma enc_dec_fw_final (t : port * port * univ) :
+  dec_fw_state_final (FwStateFinal t) = Some t.
+proof. done. qed.
+
+op is_fw_state_final (st : fw_state) : bool =
+  dec_fw_state_final st <> None.
+
+lemma is_fw_state_final (t : port * port * univ) :
+  is_fw_state_final (FwStateFinal t).
 proof. done. qed.
 
 module Forw : FUNC = {
@@ -339,8 +355,8 @@ module Forw : FUNC = {
     var r : msg option <- None;
     if (st = FwStateInit) {
       if (is_fw_req m) {
-        (addr1, pt1, pt2, u) <- oget(dec_fw_req m);
-        if (self = addr1 /\ ! self <= pt2.`1 /\ ! self <= pt2.`1) {
+        (addr1, pt1, pt2, u) <- oget (dec_fw_req m);
+        if (self = addr1 /\ ! self <= pt1.`1 /\ ! self <= pt2.`1) {
           r <- Some (fw_obs self adv pt1 pt2 u);
           st <- FwStateWait (pt1, pt2, u);
         }
@@ -351,9 +367,8 @@ module Forw : FUNC = {
       if (is_fw_ok m) {
         (addr1, addr2) <- oget (dec_fw_ok m);
         if (addr1 = self) {
-          (pt1, pt2, u) <- oget (dec_fw_state_wait st);
           r <- Some (fw_rsp self pt1 pt2 u);
-          st <- FwStateFinal;
+          st <- FwStateFinal (pt1, pt2, u);
         }
       }
     }
@@ -367,12 +382,12 @@ theory KeyExchange.
 
 (* theory parameters *)
 
-(* port index of adversary that key exchange functionalities
-   communicate with *)
+(* port index of adversary that forwarding functionalities communicate
+   with *)
 
 op adv_fw_pi : int.
 
-(* port index of adversary that simulator communicates with *)
+(* port index of adversary for key exchange simulator *)
 
 op ke_sim_adv_pi : int.
 
@@ -419,7 +434,7 @@ op dec_ke_rsp1 (m : msg) : (addr * port * port * bits) option =
            let b = oget (dec_univ_base v2)
            in (! is_base_bits b) ?
               None :
-              Some (pt2.`1, oget(dec_univ_port v1), pt1, oget (dec_base_bits b)).
+              Some (pt2.`1, oget (dec_univ_port v1), pt1, oget (dec_base_bits b)).
 
 lemma enc_dec_ke_rsp1 (func : addr, pt1 pt2 : port, x : bits) :
   dec_ke_rsp1 (ke_rsp1 func pt1 pt2 x) = Some (func, pt1, pt2, x).
@@ -505,127 +520,145 @@ realize fwd_pi_uniq. by have := ke_pi_uniq. qed.
 
 type ke_real_state = [
     KERealStateWaitReq1
-  | KERealStateWaitFwd1 of (port * port)
-  | KERealStateWaitReq2 of (port * port)
-  | KERealStateWaitFwd2 of (port * port)
-  | KERealStateFinal
+  | KERealStateWaitFwd1 of (port * port * exp)
+  | KERealStateWaitReq2 of (port * port * exp * exp)
+  | KERealStateWaitFwd2 of (port * port * exp * exp)
+  | KERealStateFinal    of (port * port * exp * exp)
 ].
 
-op dec_ke_real_state_wait_fwd1 (st : ke_real_state) : (port * port) option =
+op dec_ke_real_state_wait_fwd1 (st : ke_real_state) :
+     (port * port * exp) option =
      with st = KERealStateWaitReq1   => None
-     with st = KERealStateWaitFwd1 p => Some p
+     with st = KERealStateWaitFwd1 x => Some x
      with st = KERealStateWaitReq2 _ => None
      with st = KERealStateWaitFwd2 _ => None
-     with st = KERealStateFinal      => None.
+     with st = KERealStateFinal _    => None.
 
-lemma enc_dec_ke_real_state_wait_fwd1 (p : port * port) :
-  dec_ke_real_state_wait_fwd1 (KERealStateWaitFwd1 p) = Some p.
+lemma enc_dec_ke_real_state_wait_fwd1 (x : port * port * exp) :
+  dec_ke_real_state_wait_fwd1 (KERealStateWaitFwd1 x) = Some x.
 proof. done. qed.
 
 op is_ke_real_state_wait_fwd1 (st : ke_real_state) : bool =
   dec_ke_real_state_wait_fwd1 st <> None.
 
-lemma is_ke_real_state_wait_fwd1 (p : port * port) :
-  is_ke_real_state_wait_fwd1 (KERealStateWaitFwd1 p).
+lemma is_ke_real_state_wait_fwd1 (x : port * port * exp) :
+  is_ke_real_state_wait_fwd1 (KERealStateWaitFwd1 x).
 proof. done. qed.
 
-op dec_ke_real_state_wait_req2 (st : ke_real_state) : (port * port) option =
+op dec_ke_real_state_wait_req2 (st : ke_real_state) :
+     (port * port * exp * exp) option =
      with st = KERealStateWaitReq1   => None
      with st = KERealStateWaitFwd1 _ => None
-     with st = KERealStateWaitReq2 p => Some p
+     with st = KERealStateWaitReq2 x => Some x
      with st = KERealStateWaitFwd2 _ => None
-     with st = KERealStateFinal      => None.
+     with st = KERealStateFinal _    => None.
 
-lemma enc_dec_ke_real_state_wait_req2 (p : port * port) :
-  dec_ke_real_state_wait_req2 (KERealStateWaitReq2 p) = Some p.
+lemma enc_dec_ke_real_state_wait_req2 (x : port * port * exp * exp) :
+  dec_ke_real_state_wait_req2 (KERealStateWaitReq2 x) = Some x.
 proof. done. qed.
 
 op is_ke_real_state_wait_req2 (st : ke_real_state) : bool =
   dec_ke_real_state_wait_req2 st <> None.
 
-lemma is_ke_real_state_wait_req2 (p : port * port) :
-  is_ke_real_state_wait_req2 (KERealStateWaitReq2 p).
+lemma is_ke_real_state_wait_req2 (x : port * port * exp * exp) :
+  is_ke_real_state_wait_req2 (KERealStateWaitReq2 x).
 proof. done. qed.
 
-op dec_ke_real_state_wait_fwd2 (st : ke_real_state) : (port * port) option =
+op dec_ke_real_state_wait_fwd2 (st : ke_real_state) :
+     (port * port * exp * exp) option =
      with st = KERealStateWaitReq1   => None
      with st = KERealStateWaitFwd1 _ => None
      with st = KERealStateWaitReq2 _ => None
-     with st = KERealStateWaitFwd2 p => Some p
-     with st = KERealStateFinal      => None.
+     with st = KERealStateWaitFwd2 x => Some x
+     with st = KERealStateFinal _    => None.
 
-lemma enc_dec_ke_real_state_wait_fwd2 (p : port * port) :
-  dec_ke_real_state_wait_fwd2 (KERealStateWaitFwd2 p) = Some p.
+lemma enc_dec_ke_real_state_wait_fwd2 (x : port * port * exp * exp) :
+  dec_ke_real_state_wait_fwd2 (KERealStateWaitFwd2 x) = Some x.
 proof. done. qed.
 
 op is_ke_real_state_wait_fwd2 (st : ke_real_state) : bool =
   dec_ke_real_state_wait_fwd2 st <> None.
 
-lemma is_ke_real_state_wait_fwd2 (p : port * port) :
-  is_ke_real_state_wait_fwd2 (KERealStateWaitFwd2 p).
+lemma is_ke_real_state_wait_fwd2 (x : port * port * exp * exp) :
+  is_ke_real_state_wait_fwd2 (KERealStateWaitFwd2 x).
+proof. done. qed.
+
+op dec_ke_real_state_final (st : ke_real_state) :
+     (port * port * exp * exp) option =
+     with st = KERealStateWaitReq1   => None
+     with st = KERealStateWaitFwd1 _ => None
+     with st = KERealStateWaitReq2 _ => None
+     with st = KERealStateWaitFwd2 _ => None
+     with st = KERealStateFinal x    => Some x.
+
+lemma enc_dec_ke_real_state_final (x : port * port * exp * exp) :
+  dec_ke_real_state_final (KERealStateFinal x) = Some x.
+proof. done. qed.
+
+op is_ke_real_state_final (st : ke_real_state) : bool =
+  dec_ke_real_state_final st <> None.
+
+lemma is_ke_real_state_final (x : port * port * exp * exp) :
+  is_ke_real_state_final (KERealStateFinal x).
 proof. done. qed.
 
 module KEReal : FUNC = {
   var self, adv : addr
-  var q1, q2 : exp
   var st : ke_real_state
 
   proc init(self_ adv_ : addr) : unit = {
     self <- self_; adv <- adv_;
     Fwd1.Forw.init(self ++ [1], adv); Fwd2.Forw.init(self ++ [2], adv);
-    q1 <$ dexp; q2 <$ dexp;
     st <- KERealStateWaitReq1;
   }
 
   proc parties(m : msg) : msg option = {
     var pt1, pt2, pt1', pt2' : port; var addr : addr;
-    var u : univ; var b1, b2 : base; var x1, x2 : bits;
+    var u : univ; var x1, x2 : bits; var q1, q2 : exp;
     var r : msg option <- None;
     if (st = KERealStateWaitReq1) {  (* P1 can respond *)
       if (is_ke_req1 m) {
         (addr, pt1, pt2) <- oget (dec_ke_req1 m);
         if (! self <= pt1.`1 /\ ! self <= pt2.`1) {
+          q1 <$ dexp;
           r <-
             Some (Fwd1.fw_req (self ++ [1]) (self, 1) (self, 2)
                               (UnivBase (BaseBits (g ^ q1))));
-          st <- KERealStateWaitFwd1(pt1, pt2);
+          st <- KERealStateWaitFwd1 (pt1, pt2, q1);
         }
       }
     }
     elif (is_ke_real_state_wait_fwd1 st) {  (* P2 can respond *)
-      (pt1, pt2) <- oget (dec_ke_real_state_wait_fwd1 st);
+      (pt1, pt2, q1) <- oget (dec_ke_real_state_wait_fwd1 st);
       if (Fwd1.is_fw_rsp m) {
         (addr, pt1', pt2', u) <- oget (Fwd1.dec_fw_rsp m);
-        if (addr = self ++ [1]) {
-          b1 <- oget (dec_univ_base (oget (dec_univ_pair u)).`2);
-          x1 <- oget (dec_base_bits b1);
-          r <- Some (ke_rsp1 self pt1 pt2 (x1 ^ q2));
-          st <- KERealStateWaitReq2(pt1, pt2);
-        }
+        (* addr = self ++ [1], pt1' = (self, 1), pt2' = (self, 2) *)
+        x1 <- oget (dec_base_bits (oget (dec_univ_base u)));
+        q2 <$ dexp;
+        r <- Some (ke_rsp1 self pt1 pt2 (x1 ^ q2));
+        st <- KERealStateWaitReq2 (pt1, pt2, q1, q2);
       }
     }
     elif (is_ke_real_state_wait_req2 st) {  (* P2 can respond *)
-      (pt1, pt2) <- oget (dec_ke_real_state_wait_req2 st);
+      (pt1, pt2, q1, q2) <- oget (dec_ke_real_state_wait_req2 st);
       if (is_ke_req2 m) {
         (addr, pt2') <- oget (dec_ke_req2 m);
         if (pt2' = pt2) {
           r <-
             Some (Fwd2.fw_req (self ++ [2]) (self, 2) (self, 1)
                               (UnivBase (BaseBits (g ^ q2))));
-          st <- KERealStateWaitFwd2(pt1, pt2);
+          st <- KERealStateWaitFwd2 (pt1, pt2, q1, q2);
         }
       }
     }
     elif (is_ke_real_state_wait_fwd2 st) {  (* P1 can respond *)
-      (pt1, pt2) <- oget (dec_ke_real_state_wait_fwd2 st);
+      (pt1, pt2, q1, q2) <- oget (dec_ke_real_state_wait_fwd2 st);
       if (Fwd2.is_fw_rsp m) {
         (addr, pt1', pt2', u) <- oget (Fwd2.dec_fw_rsp m);
-        if (addr = self ++ [2]) {
-          b2 <- oget (dec_univ_base (oget (dec_univ_pair u)).`2);
-          x2 <- oget (dec_base_bits b2);
-          r <- Some (ke_rsp2 self pt1 (x2 ^ q1));
-          st <- KERealStateFinal;
-        }
+        (* addr = self ++ [2], pt1' = (self, 2), pt2' = (self, 1) *)
+        x2 <- oget (dec_base_bits (oget (dec_univ_base u)));
+        r <- Some (ke_rsp2 self pt1 (x2 ^ q1));
+        st <- KERealStateFinal (pt1, pt2, q1, q2);
       }
     }
     else {  (* st = KERealStateFinal *)
@@ -646,6 +679,7 @@ module KEReal : FUNC = {
       else {  (* self ++ [2] <= m.`2.`1 *)
         r <- Fwd2.Forw.invoke(m);
       }
+
       if (r = None \/ ! self <= (oget r).`2.`1) {
         not_done <- false;
       }
@@ -661,7 +695,7 @@ module KEReal : FUNC = {
     var addr1, addr2 : addr; var n1, n2 : int;
     var r : msg option <- None;
     (mod, pt1, pt2, u) <- m;
-    (addr1, n1) <- pt1; (addr2, n2) <- pt2;
+    (addr1, n1) <- pt1;
     if ((mod = Dir /\ addr1 = self) \/
         (mod = Adv /\ (self ++ [1] <= addr1 \/ self ++ [2] <= addr1))) {
       r <- loop(m);
@@ -772,113 +806,135 @@ proof. done. qed.
 
 type ke_ideal_state = [
     KEIdealStateWaitReq1
-  | KEIdealStateWaitSim1 of (port * port)
-  | KEIdealStateWaitReq2 of (port * port)
-  | KEIdealStateWaitSim2 of (port * port)
-  | KEIdealStateFinal
+  | KEIdealStateWaitSim1 of (port * port * exp)
+  | KEIdealStateWaitReq2 of (port * port * exp)
+  | KEIdealStateWaitSim2 of (port * port * exp)
+  | KEIdealStateFinal    of (port * port * exp)
 ].
 
-op dec_ke_ideal_state_wait_sim1 (st : ke_ideal_state) : (port * port) option =
+op dec_ke_ideal_state_wait_sim1 (st : ke_ideal_state) :
+     (port * port * exp) option =
      with st = KEIdealStateWaitReq1   => None
-     with st = KEIdealStateWaitSim1 p => Some p
+     with st = KEIdealStateWaitSim1 x => Some x
      with st = KEIdealStateWaitReq2 _ => None
      with st = KEIdealStateWaitSim2 _ => None
-     with st = KEIdealStateFinal      => None.
+     with st = KEIdealStateFinal _    => None.
 
-lemma enc_dec_ke_ideal_state_wait_sim1 (p : port * port) :
-  dec_ke_ideal_state_wait_sim1 (KEIdealStateWaitSim1 p) = Some p.
+lemma enc_dec_ke_ideal_state_wait_sim1 (x : port * port * exp) :
+  dec_ke_ideal_state_wait_sim1 (KEIdealStateWaitSim1 x) = Some x.
 proof. done. qed.
 
 op is_ke_ideal_state_wait_sim1 (st : ke_ideal_state) : bool =
   dec_ke_ideal_state_wait_sim1 st <> None.
 
-lemma is_ke_ideal_state_wait_sim1 (p : port * port) :
-  is_ke_ideal_state_wait_sim1 (KEIdealStateWaitSim1 p).
+lemma is_ke_ideal_state_wait_sim1 (x : port * port * exp) :
+  is_ke_ideal_state_wait_sim1 (KEIdealStateWaitSim1 x).
 proof. done. qed.
 
-op dec_ke_ideal_state_wait_req2 (st : ke_ideal_state) : (port * port) option =
+op dec_ke_ideal_state_wait_req2 (st : ke_ideal_state) :
+     (port * port * exp) option =
      with st = KEIdealStateWaitReq1   => None
      with st = KEIdealStateWaitSim1 _ => None
-     with st = KEIdealStateWaitReq2 p => Some p
+     with st = KEIdealStateWaitReq2 x => Some x
      with st = KEIdealStateWaitSim2 _ => None
-     with st = KEIdealStateFinal      => None.
+     with st = KEIdealStateFinal _    => None.
 
-lemma enc_dec_ke_ideal_state_wait_req2 (p : port * port) :
-  dec_ke_ideal_state_wait_req2 (KEIdealStateWaitReq2 p) = Some p.
+lemma enc_dec_ke_ideal_state_wait_req2 (x : port * port * exp) :
+  dec_ke_ideal_state_wait_req2 (KEIdealStateWaitReq2 x) = Some x.
 proof. done. qed.
 
 op is_ke_ideal_state_wait_req2 (st : ke_ideal_state) : bool =
   dec_ke_ideal_state_wait_req2 st <> None.
 
-lemma is_ke_ideal_state_wait_req2 (p : port * port) :
-  is_ke_ideal_state_wait_req2 (KEIdealStateWaitReq2 p).
+lemma is_ke_ideal_state_wait_req2 (x : port * port * exp) :
+  is_ke_ideal_state_wait_req2 (KEIdealStateWaitReq2 x).
 proof. done. qed.
 
-op dec_ke_ideal_state_wait_sim2 (st : ke_ideal_state) : (port * port) option =
+op dec_ke_ideal_state_wait_sim2 (st : ke_ideal_state) :
+     (port * port * exp) option =
      with st = KEIdealStateWaitReq1   => None
      with st = KEIdealStateWaitSim1 _ => None
      with st = KEIdealStateWaitReq2 _ => None
-     with st = KEIdealStateWaitSim2 p => Some p
-     with st = KEIdealStateFinal      => None.
+     with st = KEIdealStateWaitSim2 x => Some x
+     with st = KEIdealStateFinal _    => None.
 
-lemma enc_dec_ke_ideal_state_wait_sim2 (p : port * port) :
-  dec_ke_ideal_state_wait_sim2 (KEIdealStateWaitSim2 p) = Some p.
+lemma enc_dec_ke_ideal_state_wait_sim2 (x : port * port * exp) :
+  dec_ke_ideal_state_wait_sim2 (KEIdealStateWaitSim2 x) = Some x.
 proof. done. qed.
 
 op is_ke_ideal_state_wait_sim2 (st : ke_ideal_state) : bool =
   dec_ke_ideal_state_wait_sim2 st <> None.
 
-lemma is_ke_ideal_state_wait_sim2 (p : port * port) :
-  is_ke_ideal_state_wait_sim2 (KEIdealStateWaitSim2 p).
+lemma is_ke_ideal_state_wait_sim2 (x : port * port * exp) :
+  is_ke_ideal_state_wait_sim2 (KEIdealStateWaitSim2 x).
+proof. done. qed.
+
+op dec_ke_ideal_state_final (st : ke_ideal_state) :
+     (port * port * exp) option =
+     with st = KEIdealStateWaitReq1   => None
+     with st = KEIdealStateWaitSim1 _ => None
+     with st = KEIdealStateWaitReq2 _ => None
+     with st = KEIdealStateWaitSim2 _ => None
+     with st = KEIdealStateFinal x    => Some x.
+
+lemma enc_dec_ke_ideal_state_final (x : port * port * exp) :
+  dec_ke_ideal_state_final (KEIdealStateFinal x) = Some x.
+proof. done. qed.
+
+op is_ke_ideal_state_final (st : ke_ideal_state) : bool =
+  dec_ke_ideal_state_final st <> None.
+
+lemma is_ke_ideal_state_final (x : port * port * exp) :
+  is_ke_ideal_state_final (KEIdealStateFinal x).
 proof. done. qed.
 
 module KEIdeal : FUNC = {
   var self, adv : addr
-  var q : exp
   var st : ke_ideal_state
 
   proc init(self_ adv_ : addr) : unit = {
     self <- self_; adv <- adv_;
-    q <$ dexp;
     st <- KEIdealStateWaitReq1;
   }
 
   proc parties(m : msg) : msg option = {
     var pt1, pt2, pt2' : port; var addr1, addr2 : addr;
+    var q : exp;
     var r : msg option <- None;
     if (st = KEIdealStateWaitReq1) {  (* P1 can respond *)
       if (is_ke_req1 m) {
         (addr1, pt1, pt2) <- oget (dec_ke_req1 m);
         if (! self <= pt1.`1 /\ ! self <= pt2.`1) {
+          q <$ dexp;
           r <- Some (ke_sim_req1 self adv);
-          st <- KEIdealStateWaitSim1(pt1, pt2);
+          st <- KEIdealStateWaitSim1 (pt1, pt2, q);
         }
       }
     }
     elif (is_ke_ideal_state_wait_sim1 st) {  (* P2 can respond *)
-      (pt1, pt2) <- oget (dec_ke_ideal_state_wait_sim1 st);
+      (pt1, pt2, q) <- oget (dec_ke_ideal_state_wait_sim1 st);
       if (is_ke_sim_rsp1 m) {
         (addr1, addr2) <- oget (dec_ke_sim_rsp1 m);
         r <- Some (ke_rsp1 self pt1 pt2 (g ^ q));
-        st <- KEIdealStateWaitReq2(pt1, pt2);
+        st <- KEIdealStateWaitReq2 (pt1, pt2, q);
       }
     }
     elif (is_ke_ideal_state_wait_req2 st) {  (* P2 can respond *)
-      (pt1, pt2) <- oget (dec_ke_ideal_state_wait_req2 st);
+      (pt1, pt2, q) <- oget (dec_ke_ideal_state_wait_req2 st);
       if (is_ke_req2 m) {
         (addr1, pt2') <- oget (dec_ke_req2 m);
         if (pt2' = pt2) {
           r <- Some (ke_sim_req2 self adv);
-          st <- KEIdealStateWaitSim2(pt1, pt2);
+          st <- KEIdealStateWaitSim2 (pt1, pt2, q);
         }
       }
     }
     elif (is_ke_ideal_state_wait_sim2 st) {  (* P1 can respond *)
-      (pt1, pt2) <- oget (dec_ke_ideal_state_wait_sim2 st);
+      (pt1, pt2, q) <- oget (dec_ke_ideal_state_wait_sim2 st);
       if (is_ke_sim_rsp2 m) {
         (addr1, addr2) <- oget (dec_ke_sim_rsp2 m);
         r <- Some (ke_rsp2 self pt1 (g ^ q));
-        st <- KEIdealStateFinal;
+        st <- KEIdealStateFinal (pt1, pt2, q);
       }
     }
     else {  (* st = KEIdealStateFinal *)
@@ -891,8 +947,8 @@ module KEIdeal : FUNC = {
     var addr1, addr2 : addr; var n1, n2 : int;
     var r : msg option <- None;
     (mod, pt1, pt2, u) <- m;
-    (addr1, n1) <- pt1; (addr2, n2) <- pt2;
-    if (addr1 = self /\ (n1 = 1 \/ n1 = 2)) {
+    (addr1, n1) <- pt1;
+    if (mod = Dir /\ addr1 = self) {
       r <- parties(m);
     }
     return r;
@@ -901,81 +957,100 @@ module KEIdeal : FUNC = {
 
 type ke_sim_state = [
     KESimStateWaitReq1
-  | KESimStateWaitAdv1 of addr
-  | KESimStateWaitReq2 of addr
-  | KESimStateWaitAdv2 of addr
-  | KESimStateFinal
+  | KESimStateWaitAdv1 of (addr * exp)
+  | KESimStateWaitReq2 of (addr * exp * exp)
+  | KESimStateWaitAdv2 of (addr * exp * exp)
+  | KESimStateFinal    of (addr * exp * exp)
 ].
 
-op dec_ke_sim_state_wait_adv1 (st : ke_sim_state) : addr option =
+op dec_ke_sim_state_wait_adv1 (st : ke_sim_state) : (addr * exp) option =
      with st = KESimStateWaitReq1   => None
      with st = KESimStateWaitAdv1 x => Some x
      with st = KESimStateWaitReq2 _ => None
      with st = KESimStateWaitAdv2 _ => None
-     with st = KESimStateFinal      => None.
+     with st = KESimStateFinal _    => None.
 
-lemma enc_dec_ke_sim_state_wait_adv1 (x : addr) :
+lemma enc_dec_ke_sim_state_wait_adv1 (x : addr * exp) :
   dec_ke_sim_state_wait_adv1 (KESimStateWaitAdv1 x) = Some x.
 proof. done. qed.
 
 op is_ke_sim_state_wait_adv1 (st : ke_sim_state) : bool =
   dec_ke_sim_state_wait_adv1 st <> None.
 
-lemma is_ke_sim_state_wait_adv1 (x : addr) :
+lemma is_ke_sim_state_wait_adv1 (x : addr * exp) :
   is_ke_sim_state_wait_adv1 (KESimStateWaitAdv1 x).
 proof. done. qed.
 
-op dec_ke_sim_state_wait_req2 (st : ke_sim_state) : addr option =
+op dec_ke_sim_state_wait_req2 (st : ke_sim_state) :
+     (addr * exp * exp) option =
      with st = KESimStateWaitReq1   => None
      with st = KESimStateWaitAdv1 _ => None
      with st = KESimStateWaitReq2 x => Some x
      with st = KESimStateWaitAdv2 _ => None
-     with st = KESimStateFinal      => None.
+     with st = KESimStateFinal _    => None.
 
-lemma enc_dec_ke_sim_state_wait_req2 (x : addr) :
+lemma enc_dec_ke_sim_state_wait_req2 (x : addr * exp * exp) :
   dec_ke_sim_state_wait_req2 (KESimStateWaitReq2 x) = Some x.
 proof. done. qed.
 
 op is_ke_sim_state_wait_req2 (st : ke_sim_state) : bool =
   dec_ke_sim_state_wait_req2 st <> None.
 
-lemma is_ke_sim_state_wait_req2 (x : addr) :
+lemma is_ke_sim_state_wait_req2 (x : addr * exp * exp) :
   is_ke_sim_state_wait_req2 (KESimStateWaitReq2 x).
 proof. done. qed.
 
-op dec_ke_sim_state_wait_adv2 (st : ke_sim_state) : addr option =
+op dec_ke_sim_state_wait_adv2 (st : ke_sim_state) :
+     (addr * exp * exp) option =
      with st = KESimStateWaitReq1   => None
      with st = KESimStateWaitAdv1 _ => None
      with st = KESimStateWaitReq2 _ => None
      with st = KESimStateWaitAdv2 x => Some x
-     with st = KESimStateFinal      => None.
+     with st = KESimStateFinal _    => None.
 
-lemma enc_dec_ke_sim_state_wait_adv2 (x : addr) :
+lemma enc_dec_ke_sim_state_wait_adv2 (x : addr * exp * exp) :
   dec_ke_sim_state_wait_adv2 (KESimStateWaitAdv2 x) = Some x.
 proof. done. qed.
 
 op is_ke_sim_state_wait_adv2 (st : ke_sim_state) : bool =
   dec_ke_sim_state_wait_adv2 st <> None.
 
-lemma is_ke_sim_state_wait_adv2 (x : addr) :
+lemma is_ke_sim_state_wait_adv2 (x : addr * exp * exp) :
   is_ke_sim_state_wait_adv2 (KESimStateWaitAdv2 x).
+proof. done. qed.
+
+op dec_ke_sim_state_final (st : ke_sim_state) :
+     (addr * exp * exp) option =
+     with st = KESimStateWaitReq1   => None
+     with st = KESimStateWaitAdv1 _ => None
+     with st = KESimStateWaitReq2 _ => None
+     with st = KESimStateWaitAdv2 _ => None
+     with st = KESimStateFinal x    => Some x.
+
+lemma enc_dec_ke_sim_state_final (x : addr * exp * exp) :
+  dec_ke_sim_state_final (KESimStateFinal x) = Some x.
+proof. done. qed.
+
+op is_ke_sim_state_final (st : ke_sim_state) : bool =
+  dec_ke_sim_state_final st <> None.
+
+lemma is_ke_sim_state_final (x : addr * exp * exp) :
+  is_ke_sim_state_final (KESimStateFinal x).
 proof. done. qed.
 
 module KESim (Adv : FUNC) = {
   var self, adv : addr
-  var q1, q2 : exp
   var st : ke_sim_state
 
   proc init(self_ adv_ : addr) : unit = {
     self <- self_; adv <- adv_;
     Adv.init(self, adv);
-    q1 <$ dexp; q2 <$ dexp;
     st <- KESimStateWaitReq1;
   }
 
   proc loop(m : msg) : msg option = {
     var mod : mode; var pt1, pt2 : port; var u : univ;
-    var addr, addr1, addr2 : addr;
+    var addr, addr1, addr2 : addr; var q1, q2 : exp;
     var r : msg option <- None;
     var not_done : bool <- true;
     while (not_done) {
@@ -986,20 +1061,21 @@ module KESim (Adv : FUNC) = {
         if (st = KESimStateWaitReq1) {
           if (is_ke_sim_req1 m) {
             (addr1, addr2) <- oget (dec_ke_sim_req1 m);
+            q1 <$ dexp;
             r <-
               Some (Fwd1.fw_obs (addr1 ++ [1]) self (addr1, 1) (addr1, 2)
                     (UnivBase (BaseBits (g ^ q1))));
-            st <- KESimStateWaitAdv1 addr1;
+            st <- KESimStateWaitAdv1 (addr1, q1);
           }
         }
         elif (is_ke_sim_state_wait_req2 st) {
-          addr <- oget (dec_ke_sim_state_wait_req2 st);
+          (addr, q1, q2) <- oget (dec_ke_sim_state_wait_req2 st);
           if (is_ke_sim_req2 m) {
             (addr1, addr2) <- oget (dec_ke_sim_req2 m);
             r <-
               Some (Fwd2.fw_obs (addr ++ [2]) self (addr, 2) (addr, 1)
                     (UnivBase (BaseBits (g ^ q2))));
-            st <- KESimStateWaitAdv2 addr;
+            st <- KESimStateWaitAdv2 (addr, q1, q2);
           }
         }
         if (r = None) {
@@ -1018,38 +1094,38 @@ module KESim (Adv : FUNC) = {
           m <- oget r;
           (mod, pt1, pt2, u) <- m;
           if (is_ke_sim_state_wait_adv1 st) {
-            addr <- oget (dec_ke_sim_state_wait_adv1 st);
+            (addr, q1) <- oget (dec_ke_sim_state_wait_adv1 st);
             r <- None;
             if (Fwd1.is_fw_ok m) {
               (addr1, addr2) <- oget (Fwd1.dec_fw_ok m);
               if (addr1 = addr ++ [1]) {
+                q2 <$ dexp;
                 r <- Some (ke_sim_rsp1 addr self);
-                st <- KESimStateWaitReq2 addr;
+                st <- KESimStateWaitReq2 (addr, q1, q2);
               }
             }
           }
           elif (is_ke_sim_state_wait_adv2 st) {
             r <- None;
-            addr <- oget (dec_ke_sim_state_wait_adv2 st);
+            (addr, q1, q2) <- oget (dec_ke_sim_state_wait_adv2 st);
             if (Fwd2.is_fw_ok m) {
               (addr1, addr2) <- oget (Fwd2.dec_fw_ok m);
               if (addr1 = addr ++ [2]) {
                 r <- Some (ke_sim_rsp2 addr self);
-                st <- KESimStateFinal;
+                st <- KESimStateFinal (addr, q1, q2);
               }
             }
           }
-          elif (self <= pt1.`1) {  (* not waiting on adversary *)
-            r <- None;
+          else {  (* not waiting on adversary *)
+            not_done <- false;
           }
-          not_done <- false;
         }
       }
     }
     return r;
   }  
 
-proc invoke(m : msg) : msg option = {
+  proc invoke(m : msg) : msg option = {
     var mod : mode; var pt1, pt2 : port; var u : univ;
     var r : msg option <- None;
     (mod, pt1, pt2, u) <- m;
@@ -1071,15 +1147,15 @@ module DDH_Adv (Env : ENV, Adv : FUNC) = {
 
 section.
 
-declare module Adv : FUNC{KEReal, KEIdeal, KESim, DDH_Adv}.
-declare module Env : ENV{Adv, KEReal, KEIdeal, KESim, DDH_Adv}.
+declare module Adv : FUNC{MI, KEReal, KEIdeal, KESim, DDH_Adv}.
+declare module Env : ENV{Adv, MI, KEReal, KEIdeal, KESim, DDH_Adv}.
 
-lemma KESec (func adv : addr) &m :
+lemma ke_sec (func adv : addr) &m :
   exper_pre func adv (fset1 adv_fw_pi) =>
   DDH_Adv.func{m} = func => DDH_Adv.adv{m} = adv =>
-  `|Pr[Exper(MakeInter(KEReal, Adv), Env).main
+  `|Pr[Exper(MI(KEReal, Adv), Env).main
          (func, adv, fset1 adv_fw_pi) @ &m : res] -
-    Pr[Exper(MakeInter(KEIdeal, KESim(Adv)), Env).main
+    Pr[Exper(MI(KEIdeal, KESim(Adv)), Env).main
          (func, adv, fset1 adv_fw_pi) @ &m : res]| <=
   `|Pr[DDH1(DDH_Adv(Env, Adv)).main() @ &m : res] -
     Pr[DDH2(DDH_Adv(Env, Adv)).main() @ &m : res]|.
@@ -1089,21 +1165,21 @@ qed.
 
 end section.
 
-lemma KESecurity
-        (Adv <: FUNC{KEReal, KEIdeal, KESim, DDH_Adv})
-        (Env <: ENV{Adv, KEReal, KEIdeal, KESim, DDH_Adv})
+lemma ke_security
+        (Adv <: FUNC{MI, KEReal, KEIdeal, KESim, DDH_Adv})
+        (Env <: ENV{Adv, MI, KEReal, KEIdeal, KESim, DDH_Adv})
         (func adv : addr) &m :
   exper_pre func adv (fset1 adv_fw_pi) =>
   DDH_Adv.func{m} = func => DDH_Adv.adv{m} = adv =>
-  `|Pr[Exper(MakeInter(KEReal, Adv), Env).main
+  `|Pr[Exper(MI(KEReal, Adv), Env).main
          (func, adv, fset1 adv_fw_pi) @ &m : res] -
-    Pr[Exper(MakeInter(KEIdeal, KESim(Adv)), Env).main
+    Pr[Exper(MI(KEIdeal, KESim(Adv)), Env).main
          (func, adv, fset1 adv_fw_pi) @ &m : res]| <=
   `|Pr[DDH1(DDH_Adv(Env, Adv)).main() @ &m : res] -
     Pr[DDH2(DDH_Adv(Env, Adv)).main() @ &m : res]|.
 proof.
 move => pre func_eq adv_eq.
-by apply (KESec Adv Env func adv &m).
+by apply (ke_sec Adv Env func adv &m).
 qed.
 
 end KeyExchange.
@@ -1117,13 +1193,11 @@ theory SMC.
 
 op adv_fw_pi : int.
 
-(* port index of adversary that key exchange's simulator communicates
-   with *)
+(* port index of adversary for key exchange's simulator *)
 
 op ke_sim_adv_pi : int.
 
-(* port index of adversary that SMC's simulator communicates
-   with *)
+(* port index of adversary for SMC's simulator *)
 
 op smc_sim_adv_pi : int.
 
@@ -1184,7 +1258,7 @@ op dec_smc_rsp (m : msg) : (addr * port * port * bits) option =
            let b = oget (dec_univ_base v2)
            in (! is_base_bits b) ?
               None :
-              Some (pt2.`1, oget(dec_univ_port v1), pt1, oget (dec_base_bits b)).
+              Some (pt2.`1, oget (dec_univ_port v1), pt1, oget (dec_base_bits b)).
 
 lemma enc_dec_smc_rsp (func : addr, pt1 pt2 : port, x : bits) :
   dec_smc_rsp (smc_rsp func pt1 pt2 x) = Some (func, pt1, pt2, x).
@@ -1219,7 +1293,7 @@ type smc_real_state = [
   | SMCRealStateWaitKE1 of (port * port * bits)
   | SMCRealStateWaitKE2 of (port * port * bits * bits)
   | SMCRealStateWaitFwd of (port * port * bits * bits * bits)
-  | SMCRealStateFinal
+  | SMCRealStateFinal   of (port * port * bits * bits * bits)
 ].
 
 op dec_smc_real_state_wait_ke1 (st : smc_real_state) :
@@ -1228,7 +1302,7 @@ op dec_smc_real_state_wait_ke1 (st : smc_real_state) :
      with st = SMCRealStateWaitKE1 x => Some x
      with st = SMCRealStateWaitKE2 _ => None
      with st = SMCRealStateWaitFwd _ => None
-     with st = SMCRealStateFinal     => None.
+     with st = SMCRealStateFinal _   => None.
 
 lemma enc_dec_smc_real_state_wait_ke1 (x : port * port * bits) :
   dec_smc_real_state_wait_ke1 (SMCRealStateWaitKE1 x) = Some x.
@@ -1247,7 +1321,7 @@ op dec_smc_real_state_wait_ke2 (st : smc_real_state) :
      with st = SMCRealStateWaitKE1 _ => None
      with st = SMCRealStateWaitKE2 x => Some x
      with st = SMCRealStateWaitFwd _ => None
-     with st = SMCRealStateFinal     => None.
+     with st = SMCRealStateFinal _   => None.
 
 lemma enc_dec_smc_real_state_wait_ke2 (x : port * port * bits * bits) :
   dec_smc_real_state_wait_ke2 (SMCRealStateWaitKE2 x) = Some x.
@@ -1266,7 +1340,7 @@ op dec_smc_real_state_wait_fwd (st : smc_real_state) :
      with st = SMCRealStateWaitKE1 _ => None
      with st = SMCRealStateWaitKE2 _ => None
      with st = SMCRealStateWaitFwd x => Some x
-     with st = SMCRealStateFinal     => None.
+     with st = SMCRealStateFinal _   => None.
 
 lemma enc_dec_smc_real_state_wait_fwd (x : port * port * bits * bits * bits) :
   dec_smc_real_state_wait_fwd (SMCRealStateWaitFwd x) = Some x.
@@ -1277,6 +1351,25 @@ op is_smc_real_state_wait_fwd (st : smc_real_state) : bool =
 
 lemma is_smc_real_state_wait_fwd (x : port * port * bits * bits * bits) :
   is_smc_real_state_wait_fwd (SMCRealStateWaitFwd x).
+proof. done. qed.
+
+op dec_smc_real_state_final (st : smc_real_state) :
+     (port * port * bits * bits * bits) option =
+     with st = SMCRealStateWaitReq   => None
+     with st = SMCRealStateWaitKE1 _ => None
+     with st = SMCRealStateWaitKE2 _ => None
+     with st = SMCRealStateWaitFwd _ => None
+     with st = SMCRealStateFinal x   => Some x.
+
+lemma enc_dec_smc_real_state_final (x : port * port * bits * bits * bits) :
+  dec_smc_real_state_final (SMCRealStateFinal x) = Some x.
+proof. done. qed.
+
+op is_smc_real_state_final (st : smc_real_state) : bool =
+  dec_smc_real_state_final st <> None.
+
+lemma is_smc_real_state_final (x : port * port * bits * bits * bits) :
+  is_smc_real_state_final (SMCRealStateFinal x).
 proof. done. qed.
 
 module SMCReal (KE : FUNC) : FUNC = {
@@ -1299,7 +1392,7 @@ module SMCReal (KE : FUNC) : FUNC = {
         if (! self <= pt1.`1 /\ ! self <= pt2.`1) {
           r <-
             Some (KeyEx.ke_req1 (self ++ [2]) (self, 1) (self, 2));
-          st <- SMCRealStateWaitKE1(pt1, pt2, x1);
+          st <- SMCRealStateWaitKE1 (pt1, pt2, x1);
         }
       }
     }
@@ -1309,7 +1402,7 @@ module SMCReal (KE : FUNC) : FUNC = {
         (addr, pt1', pt2', k2) <- oget (KeyEx.dec_ke_rsp1 m);
         r <-
           Some (KeyEx.ke_req2 (self ++ [2]) (self, 2));
-        st <- SMCRealStateWaitKE2(pt1, pt2, x1, k2);
+        st <- SMCRealStateWaitKE2 (pt1, pt2, x1, k2);
       }
     }
     elif (is_smc_real_state_wait_ke2 st) {  (* P1 *)
@@ -1319,7 +1412,7 @@ module SMCReal (KE : FUNC) : FUNC = {
         r <-
           Some (Fwd.fw_req (self ++ [1]) (self, 1) (self, 2)
                 (UnivBase (BaseBits (x1 ^^ k1))));
-        st <- SMCRealStateWaitFwd(pt1, pt2, x1, k2, k1);
+        st <- SMCRealStateWaitFwd (pt1, pt2, x1, k2, k1);
       }
     }
     elif (is_smc_real_state_wait_fwd st) {  (* P2 *)
@@ -1328,7 +1421,7 @@ module SMCReal (KE : FUNC) : FUNC = {
         (addr, pt1', pt2', u) <- oget (Fwd.dec_fw_rsp m);
         x2 <- oget (dec_base_bits (oget (dec_univ_base u))) ^^ k2;
         r <- Some (smc_rsp self pt1 pt2 x2);
-        st <- SMCRealStateFinal;
+        st <- SMCRealStateFinal (pt1, pt2, x1, k2, k1);
       }
     }
     return r;
@@ -1346,6 +1439,13 @@ module SMCReal (KE : FUNC) : FUNC = {
       }
       else {  (* self ++ [2] <= m.`2.`1 *)
         r <- KE.invoke(m);
+        if (r <> None /\
+            let (mod, pt1, pt2, u) = oget r in
+            let (addr1, n1) = pt1
+            in !((mod = Dir /\ addr1 = self) \/
+                 (mod = Adv /\ ! self <= addr1))) {
+          r <- None;
+        }
       }
       if (r = None \/ ! self <= (oget r).`2.`1) {
         not_done <- false;
@@ -1422,14 +1522,14 @@ proof. done. qed.
 type smc_ideal_state = [
     SMCIdealStateWaitReq
   | SMCIdealStateWaitSim of (port * port * bits)
-  | SMCIdealStateFinal
+  | SMCIdealStateFinal   of (port * port * bits)
 ].
 
 op dec_smc_ideal_state_wait_sim (st : smc_ideal_state) :
      (port * port * bits) option =
      with st = SMCIdealStateWaitReq   => None
      with st = SMCIdealStateWaitSim x => Some x
-     with st = SMCIdealStateFinal     => None.
+     with st = SMCIdealStateFinal _   => None.
 
 lemma enc_dec_smc_ideal_state_wait_sim (x : port * port * bits) :
   dec_smc_ideal_state_wait_sim (SMCIdealStateWaitSim x) = Some x.
@@ -1442,12 +1542,28 @@ lemma is_smc_ideal_state_wait_sim (x : port * port * bits) :
   is_smc_ideal_state_wait_sim (SMCIdealStateWaitSim x).
 proof. done. qed.
 
+op dec_smc_ideal_state_final (st : smc_ideal_state) :
+     (port * port * bits) option =
+     with st = SMCIdealStateWaitReq   => None
+     with st = SMCIdealStateWaitSim _ => None
+     with st = SMCIdealStateFinal x   => Some x.
+
+lemma enc_dec_smc_ideal_state_final (x : port * port * bits) :
+  dec_smc_ideal_state_final (SMCIdealStateFinal x) = Some x.
+proof. done. qed.
+
+op is_smc_ideal_state_final (st : smc_ideal_state) : bool =
+  dec_smc_ideal_state_final st <> None.
+
+lemma is_smc_ideal_state_final (x : port * port * bits) :
+  is_smc_ideal_state_final (SMCIdealStateFinal x).
+proof. done. qed.
+
 module SMCIdeal : FUNC = {
   var self, adv : addr
   var st : smc_ideal_state
 
   proc init(self_ adv_ : addr) : unit = {
-    var u : exp;
     self <- self_; adv <- adv_;
     st <- SMCIdealStateWaitReq;
   }
@@ -1470,7 +1586,7 @@ module SMCIdeal : FUNC = {
       if (is_smc_sim_rsp m) {
         (addr1, addr2) <- oget (dec_smc_sim_rsp m);
         r <- Some (smc_rsp self pt1 pt2 x);
-        st <- SMCIdealStateFinal;
+        st <- SMCIdealStateFinal (pt1, pt2, x);
       }
     }
     return r;
@@ -1491,82 +1607,97 @@ module SMCIdeal : FUNC = {
 
 type smc_sim_state = [
     SMCSimStateWaitReq
-  | SMCSimStateWaitAdv1 of addr
-  | SMCSimStateWaitAdv2 of addr
-  | SMCSimStateWaitAdv3 of addr
-  | SMCSimStateFinal
+  | SMCSimStateWaitAdv1 of (addr * exp)
+  | SMCSimStateWaitAdv2 of (addr * exp)
+  | SMCSimStateWaitAdv3 of (addr * exp)
+  | SMCSimStateFinal    of (addr * exp)
 ].
 
-op dec_smc_sim_state_wait_adv1 (st : smc_sim_state) : addr option =
+op dec_smc_sim_state_wait_adv1 (st : smc_sim_state) : (addr * exp) option =
      with st = SMCSimStateWaitReq    => None
      with st = SMCSimStateWaitAdv1 x => Some x
      with st = SMCSimStateWaitAdv2 _ => None
      with st = SMCSimStateWaitAdv3 _ => None
-     with st = SMCSimStateFinal      => None.
+     with st = SMCSimStateFinal _    => None.
 
-lemma enc_dec_smc_sim_state_wait_adv1 (x : addr) :
+lemma enc_dec_smc_sim_state_wait_adv1 (x : addr * exp) :
   dec_smc_sim_state_wait_adv1 (SMCSimStateWaitAdv1 x) = Some x.
 proof. done. qed.
 
 op is_smc_sim_state_wait_adv1 (st : smc_sim_state) : bool =
   dec_smc_sim_state_wait_adv1 st <> None.
 
-lemma is_smc_sim_state_wait_adv1 (x : addr) :
+lemma is_smc_sim_state_wait_adv1 (x : addr * exp) :
   is_smc_sim_state_wait_adv1 (SMCSimStateWaitAdv1 x).
 proof. done. qed.
 
-op dec_smc_sim_state_wait_adv2 (st : smc_sim_state) : addr option =
+op dec_smc_sim_state_wait_adv2 (st : smc_sim_state) : (addr * exp) option =
      with st = SMCSimStateWaitReq    => None
      with st = SMCSimStateWaitAdv1 _ => None
      with st = SMCSimStateWaitAdv2 x => Some x
      with st = SMCSimStateWaitAdv3 _ => None
-     with st = SMCSimStateFinal      => None.
+     with st = SMCSimStateFinal _    => None.
 
-lemma enc_dec_smc_sim_state_wait_adv2 (x : addr) :
+lemma enc_dec_smc_sim_state_wait_adv2 (x : addr * exp) :
   dec_smc_sim_state_wait_adv2 (SMCSimStateWaitAdv2 x) = Some x.
 proof. done. qed.
 
 op is_smc_sim_state_wait_adv2 (st : smc_sim_state) : bool =
   dec_smc_sim_state_wait_adv2 st <> None.
 
-lemma is_smc_sim_state_wait_adv2 (x : addr) :
+lemma is_smc_sim_state_wait_adv2 (x : addr * exp) :
   is_smc_sim_state_wait_adv2 (SMCSimStateWaitAdv2 x).
 proof. done. qed.
 
-op dec_smc_sim_state_wait_adv3 (st : smc_sim_state) : addr option =
+op dec_smc_sim_state_wait_adv3 (st : smc_sim_state) : (addr * exp) option =
      with st = SMCSimStateWaitReq    => None
      with st = SMCSimStateWaitAdv1 _ => None
      with st = SMCSimStateWaitAdv2 _ => None
      with st = SMCSimStateWaitAdv3 x => Some x
-     with st = SMCSimStateFinal      => None.
+     with st = SMCSimStateFinal _    => None.
 
-lemma enc_dec_smc_sim_state_wait_adv3 (x : addr) :
+lemma enc_dec_smc_sim_state_wait_adv3 (x : addr * exp) :
   dec_smc_sim_state_wait_adv3 (SMCSimStateWaitAdv3 x) = Some x.
 proof. done. qed.
 
 op is_smc_sim_state_wait_adv3 (st : smc_sim_state) : bool =
   dec_smc_sim_state_wait_adv3 st <> None.
 
-lemma is_smc_sim_state_wait_adv3 (x : addr) :
+lemma is_smc_sim_state_wait_adv3 (x : addr * exp) :
   is_smc_sim_state_wait_adv3 (SMCSimStateWaitAdv3 x).
+proof. done. qed.
+
+op dec_smc_sim_state_final (st : smc_sim_state) : (addr * exp) option =
+     with st = SMCSimStateWaitReq    => None
+     with st = SMCSimStateWaitAdv1 _ => None
+     with st = SMCSimStateWaitAdv2 _ => None
+     with st = SMCSimStateWaitAdv3 _ => None
+     with st = SMCSimStateFinal x    => Some x.
+
+lemma enc_dec_smc_sim_state_final (x : addr * exp) :
+  dec_smc_sim_state_final (SMCSimStateFinal x) = Some x.
+proof. done. qed.
+
+op is_smc_sim_state_final (st : smc_sim_state) : bool =
+  dec_smc_sim_state_final st <> None.
+
+lemma is_smc_sim_state_final (x : addr * exp) :
+  is_smc_sim_state_final (SMCSimStateFinal x).
 proof. done. qed.
 
 module SMCSim (Adv : FUNC) = {
   var self, adv : addr
-  var x : bits
   var st : smc_sim_state
 
   proc init(self_ adv_ : addr) : unit = {
-    var q : exp;
     self <- self_; adv <- adv_;
     Adv.init(self, adv);
-    q <$ dexp; x <- g ^ q;
     st <- SMCSimStateWaitReq;
   }
 
   proc loop(m : msg) : msg option = {
     var mod : mode; var pt1, pt2 : port; var u : univ;
-    var addr, addr1, addr2 : addr;
+    var addr, addr1, addr2 : addr; var q : exp;
     var r : msg option <- None;
     var not_done : bool <- true;
     while (not_done) {
@@ -1577,8 +1708,9 @@ module SMCSim (Adv : FUNC) = {
         if (st = SMCSimStateWaitReq) {
           if (is_smc_sim_req m) {
             (addr1, addr2) <- oget (dec_smc_sim_req m);
+            q <$ dexp;
             r <- Some (KeyEx.ke_sim_req1 (addr1 ++ [2]) self);
-            st <- SMCSimStateWaitAdv1 addr1;
+            st <- SMCSimStateWaitAdv1 (addr1, q);
           }
         }
         if (r = None) {
@@ -1596,160 +1728,965 @@ module SMCSim (Adv : FUNC) = {
         else {
           m <- oget r; (mod, pt1, pt2, u) <- m;
           if (is_smc_sim_state_wait_adv1 st) {
-            addr <- oget (dec_smc_sim_state_wait_adv1 st);
+            (addr, q) <- oget (dec_smc_sim_state_wait_adv1 st);
             r <- None;
             if (KeyEx.is_ke_sim_rsp1 m) {
               (addr1, addr2) <- oget (KeyEx.dec_ke_sim_rsp1 m);
               if (addr1 = addr ++ [2]) {
                 r <- Some (KeyEx.ke_sim_req2 (addr ++ [2]) self);
-                st <- SMCSimStateWaitAdv2 addr;
+                st <- SMCSimStateWaitAdv2 (addr, q);
               }
             }
           }
-          if (is_smc_sim_state_wait_adv2 st) {
-            addr <- oget (dec_smc_sim_state_wait_adv2 st);
+          elif (is_smc_sim_state_wait_adv2 st) {
+            (addr, q) <- oget (dec_smc_sim_state_wait_adv2 st);
             r <- None;
             if (KeyEx.is_ke_sim_rsp2 m) {
               (addr1, addr2) <- oget (KeyEx.dec_ke_sim_rsp2 m);
               if (addr1 = addr ++ [2]) {
                 r <-
                   Some (Fwd.fw_obs (addr ++ [1]) self (addr, 1) (addr, 2)
-                        (UnivBase (BaseBits x)));
-                st <- SMCSimStateWaitAdv3 addr;
+                        (UnivBase (BaseBits (g ^ q))));
+                st <- SMCSimStateWaitAdv3 (addr, q);
               }
             }
           }
-          if (is_smc_sim_state_wait_adv3 st) {
-            addr <- oget (dec_smc_sim_state_wait_adv3 st);
+          elif (is_smc_sim_state_wait_adv3 st) {
+            (addr, q) <- oget (dec_smc_sim_state_wait_adv3 st);
             r <- None;
             if (Fwd.is_fw_ok m) {
               (addr1, addr2) <- oget (Fwd.dec_fw_ok m);
               if (addr1 = addr ++ [1]) {
                 r <- Some (smc_sim_rsp addr self);
-                st <- SMCSimStateFinal;
+                st <- SMCSimStateFinal (addr, q);
               }
             }
           }
-          elif (self <= pt1.`1) {  (* not waiting on adversary *)
-            r <- None;
+          else {  (* not waiting on adversary *)
+            not_done <- false;
           }
-          not_done <- false;
         }
       }
     }
     return r;
   }  
 
-proc invoke(m : msg) : msg option = {
-    var mod : mode; var pt1, pt2 : port; var u : univ;
-    var r : msg option <- None;
-    (mod, pt1, pt2, u) <- m;
-    if (mod = Adv /\ pt1.`1 = self) {
-      r <- loop(m);
+  proc invoke(m : msg) : msg option = {
+      var mod : mode; var pt1, pt2 : port; var u : univ;
+      var r : msg option <- None;
+      (mod, pt1, pt2, u) <- m;
+      if (mod = Adv /\ pt1.`1 = self) {
+        r <- loop(m);
+      }
+      return r;
     }
-    return r;
-  }
 }.
 
 module CompEnv (Env : ENV, Inter : INTER) = {
+  module Stub : FUNC = {
+    proc init(func adv : addr) : unit = { }
+
+    proc invoke(m : msg) : msg option = {
+      var r : msg option;
+      r <@ Inter.invoke(m);
+      return r;
+    }
+  }
+
+  (* func will end with 2 *)
+
   proc main(func adv : addr, in_guard : int fset) : bool = {
-    (* placeholder *)
-    return true;
+    var b : bool;
+    b <@ Exper(MI_UOC(SMCReal(Stub), Stub), Env).main
+           (take (size func - 1) func, adv, in_guard);
+    return b;
   }
 }.
 
 section.
 
-declare module Adv : FUNC{SMCReal, KeyEx.KEReal, KeyEx.KEIdeal,
-                          KeyEx.KESim, KeyEx.DDH_Adv}.
-declare module Env : ENV{Adv, SMCReal, KeyEx.KEReal, KeyEx.KEIdeal,
-                         KeyEx.KESim, KeyEx.DDH_Adv}.
+declare module Adv : FUNC{MI, SMCReal, KeyEx.KEReal, KeyEx.KEIdeal,
+                          KeyEx.DDH_Adv, CompEnv}.
+declare module Env : ENV{Adv, MI, SMCReal, KeyEx.KEReal, KeyEx.KEIdeal,
+                         KeyEx.DDH_Adv, CompEnv}.
 
-lemma SMCSec1 (func adv : addr) &m :
+(*
+type smc_sec1_ke_real_bridge_st = {
+  func  : addr;
+  smcrs : smc_real_state;
+  fws   : Fwd.fw_state;
+  
+
+}.
+
+   SMCReal.st{1} = SMCRealStateWaitReq /\
+   Fwd.Forw.st{1} = Fwd.FwStateInit /\
+   KeyEx.Fwd1.Forw.st{1} = KeyEx.Fwd1.FwStateInit /\
+   KeyEx.Fwd2.Forw.st{1} = KeyEx.Fwd2.FwStateInit ==>
+
+
+
+pred smc_sec2_rel0 (st : smc_sec2_st) =
+  (st.`smcrs = SMCRealStateWaitReq) /\
+  (st.`fws   = Fwd.FwStateInit) /\
+  (st.`keis  = KeyEx.KEIdealStateWaitReq1) /\
+  (st.`smcis = SMCIdealStateWaitReq) /\
+  (st.`smcss = SMCSimStateWaitReq).
+
+inductive smc_sec2_rel (st : smc_sec2_st) =
+    SMCSec2Rel0 of (smc_sec2_rel0 st)
+  | SMCSec2Rel1 (pt1 pt2 : port, x : bits, q : exp) of
+      (smc_sec2_rel1 st pt1 pt2 x q)
+  | SMCSec2Rel2 (pt1 pt2 : port, x : bits, q : exp) of
+      (smc_sec2_rel2 st pt1 pt2 x q)
+  | SMCSec2Rel3 (pt1 pt2 : port, x : bits, q : exp) of
+      (smc_sec2_rel3 st pt1 pt2 x q)
+  | SMCSec2Rel4 (pt1 pt2 : port, x : bits, q : exp) of
+      (smc_sec2_rel4 st pt1 pt2 x q).
+
+*)
+
+lemma smc_sec1_ke_real_bridge (func adv : addr) &m :
   exper_pre func adv (fset1 adv_fw_pi) =>
-  KeyEx.DDH_Adv.func{m} = func => KeyEx.DDH_Adv.adv{m} = adv =>
-  `|Pr[Exper(MakeInter(SMCReal(KeyEx.KEReal), Adv), Env).main
-         (func, adv, fset1 adv_fw_pi) @ &m : res] -
-    Pr[Exper(MakeInter(SMCReal(KeyEx.KEIdeal), KeyEx.KESim(Adv)), Env).main
-         (func, adv, fset1 adv_fw_pi) @ &m : res]| <=
-  `|Pr[DDH1(KeyEx.DDH_Adv(CompEnv(Env), Adv)).main() @ &m : res] -
-    Pr[DDH2(KeyEx.DDH_Adv(CompEnv(Env), Adv)).main() @ &m : res]|.
+  Pr[Exper(MI(SMCReal(KeyEx.KEReal), Adv), Env).main
+       (func, adv, fset1 adv_fw_pi) @ &m : res] =
+  Pr[Exper(MI(KeyEx.KEReal, Adv), CompEnv(Env)).main
+       (func ++ [2], adv, fset1 adv_fw_pi) @ &m : res].
 proof.
-move => pre func_eq adv_eq.
+move : func adv; move => func' adv' pre.
+byequiv => //.
+proc; inline*; wp; swap{2} 22 26; sp.
+conseq
+  (_ :
+   exper_pre func' adv' (fset1 adv_fw_pi) /\
+   ={SMCReal.self, SMCReal.adv, SMCReal.st,
+     Fwd.Forw.self, Fwd.Forw.adv, Fwd.Forw.st,
+     KeyEx.Fwd1.Forw.self, KeyEx.Fwd1.Forw.adv, KeyEx.Fwd1.Forw.st,
+     KeyEx.Fwd2.Forw.self, KeyEx.Fwd2.Forw.adv, KeyEx.Fwd2.Forw.st} /\
+   func{1} = func' /\ adv{1} = adv' /\ in_guard{1} = fset1 adv_fw_pi /\
+   func1{2} = func' /\ adv1{2} = adv' /\ in_guard1{2} = fset1 adv_fw_pi /\
+   MI.func{1} = func' /\ MI.adv{1} = adv' /\ MI.in_guard{1} = fset1 adv_fw_pi /\
+   ={func, adv, in_guard}(MI, MI_UOC) /\
+   MI.func{2} = func' ++ [2] /\ MI.adv{2} = adv' /\
+   MI.in_guard{2} = fset1 adv_fw_pi /\
+   Fwd.Forw.self{1} = func' ++ [1] /\ Fwd.Forw.adv{1} = adv' /\
+   KeyEx.Fwd1.Forw.self{1} = func' ++ [2; 1] /\ KeyEx.Fwd1.Forw.adv{1} = adv' /\
+   KeyEx.Fwd2.Forw.self{1} = func' ++ [2; 2] /\ KeyEx.Fwd2.Forw.adv{1} = adv' /\
+   SMCReal.st{1} = SMCRealStateWaitReq /\
+   Fwd.Forw.st{1} = Fwd.FwStateInit /\
+   KeyEx.Fwd1.Forw.st{1} = KeyEx.Fwd1.FwStateInit /\
+   KeyEx.Fwd2.Forw.st{1} = KeyEx.Fwd2.FwStateInit ==>
+   _).
+(progress;
+   first 4 by rewrite size_cat /= -addzA /= (take_size_cat (size func{1})));
+  by rewrite -catA.  
+seq 1 1 :
+  (exper_pre func' adv' (fset1 adv_fw_pi) /\
+   ={glob Adv,
+     SMCReal.self, SMCReal.adv, SMCReal.st,
+     Fwd.Forw.self, Fwd.Forw.adv, Fwd.Forw.st,
+     KeyEx.Fwd1.Forw.self, KeyEx.Fwd1.Forw.adv, KeyEx.Fwd1.Forw.st,
+     KeyEx.Fwd2.Forw.self, KeyEx.Fwd2.Forw.adv, KeyEx.Fwd2.Forw.st} /\
+   func{1} = func' /\ adv{1} = adv' /\ in_guard{1} = fset1 adv_fw_pi /\
+   func1{2} = func' /\ adv1{2} = adv' /\ in_guard1{2} = fset1 adv_fw_pi /\
+   MI.func{1} = func' /\ MI.adv{1} = adv' /\ MI.in_guard{1} = fset1 adv_fw_pi /\
+   ={func, adv, in_guard}(MI, MI_UOC) /\
+   MI.func{2} = func' ++ [2] /\ MI.adv{2} = adv' /\
+   MI.in_guard{2} = fset1 adv_fw_pi /\
+   Fwd.Forw.self{1} = func' ++ [1] /\ Fwd.Forw.adv{1} = adv' /\
+   KeyEx.Fwd1.Forw.self{1} = func' ++ [2; 1] /\ KeyEx.Fwd1.Forw.adv{1} = adv' /\
+   KeyEx.Fwd2.Forw.self{1} = func' ++ [2; 2] /\ KeyEx.Fwd2.Forw.adv{1} = adv' /\
+   SMCReal.st{1} = SMCRealStateWaitReq /\
+   Fwd.Forw.st{1} = Fwd.FwStateInit /\
+   KeyEx.Fwd1.Forw.st{1} = KeyEx.Fwd1.FwStateInit /\
+   KeyEx.Fwd2.Forw.st{1} = KeyEx.Fwd2.FwStateInit).
+call (_ : true); first auto.
+call
+  (_ :
+   ={glob Adv,
+     SMCReal.self, SMCReal.adv, SMCReal.st,
+     Fwd.Forw.self, Fwd.Forw.adv, Fwd.Forw.st,
+     KeyEx.Fwd1.Forw.self, KeyEx.Fwd1.Forw.adv, KeyEx.Fwd1.Forw.st,
+     KeyEx.Fwd2.Forw.self, KeyEx.Fwd2.Forw.adv, KeyEx.Fwd2.Forw.st} /\
+   exper_pre MI.func{1} MI.adv{1} MI.in_guard{1} /\
+   MI.in_guard{1} = fset1 adv_fw_pi /\
+   ={func, adv, in_guard}(MI, MI_UOC) /\
+   MI.func{2} = MI.func{1} ++ [2] /\ MI.adv{2} = MI.adv{1} /\
+   MI.in_guard{2} = fset1 adv_fw_pi /\
+   Fwd.Forw.self{1} = MI.func{1} ++ [1] /\ Fwd.Forw.adv{1} = MI.adv{1} /\
+   KeyEx.Fwd1.Forw.self{1} = MI.func{1} ++ [2; 1] /\
+   KeyEx.Fwd2.Forw.adv{1} = MI.adv{1} /\
+   KeyEx.Fwd2.Forw.self{1} = MI.func{1} ++ [2; 2] /\
+   KeyEx.Fwd1.Forw.adv{1} = MI.adv{1} /\
+   SMCReal.st{1} = SMCRealStateWaitReq /\
+   Fwd.Forw.st{1} = Fwd.FwStateInit /\
+   KeyEx.Fwd1.Forw.st{1} = KeyEx.Fwd1.FwStateInit /\
+   KeyEx.Fwd2.Forw.st{1} = KeyEx.Fwd2.FwStateInit).
+proc.
+admit.
+auto.
+qed.
+
+lemma smc_sec1_ke_ideal_bridge (func adv : addr) &m :
+  exper_pre func adv (fset1 adv_fw_pi) =>
+  Pr[Exper(MI(SMCReal(KeyEx.KEIdeal), Adv), Env).main
+       (func, adv, fset1 adv_fw_pi) @ &m : res] =
+  Pr[Exper(MI(KeyEx.KEIdeal, Adv), CompEnv(Env)).main
+       (func ++ [2], adv, fset1 adv_fw_pi) @ &m : res].
+proof.
 admit.
 qed.
 
 end section.
 
-lemma SMCSecurity1
-        (Adv <: FUNC{SMCReal, KeyEx.KEReal, KeyEx.KEIdeal,
-                     KeyEx.KESim, KeyEx.DDH_Adv})
-        (Env <: ENV{Adv, SMCReal, KeyEx.KEReal, KeyEx.KEIdeal,
-                    KeyEx.KESim, KeyEx.DDH_Adv})
-        (func adv : addr) &m :
+section.
+
+declare module Adv : FUNC{MI, SMCReal, KeyEx.KEReal, KeyEx.KEIdeal,
+                          KeyEx.KESim, KeyEx.DDH_Adv, CompEnv}.
+declare module Env : ENV{Adv, MI, SMCReal, KeyEx.KEReal, KeyEx.KEIdeal,
+                         KeyEx.KESim, KeyEx.DDH_Adv, CompEnv}.
+
+lemma smc_sec1 (func adv : addr) &m :
   exper_pre func adv (fset1 adv_fw_pi) =>
-  KeyEx.DDH_Adv.func{m} = func => KeyEx.DDH_Adv.adv{m} = adv =>
-  `|Pr[Exper(MakeInter(SMCReal(KeyEx.KEReal), Adv), Env).main
+  KeyEx.DDH_Adv.func{m} = func ++ [2] => KeyEx.DDH_Adv.adv{m} = adv =>
+  `|Pr[Exper(MI(SMCReal(KeyEx.KEReal), Adv), Env).main
          (func, adv, fset1 adv_fw_pi) @ &m : res] -
-    Pr[Exper(MakeInter(SMCReal(KeyEx.KEIdeal), KeyEx.KESim(Adv)), Env).main
+    Pr[Exper(MI(SMCReal(KeyEx.KEIdeal), KeyEx.KESim(Adv)), Env).main
          (func, adv, fset1 adv_fw_pi) @ &m : res]| <=
   `|Pr[DDH1(KeyEx.DDH_Adv(CompEnv(Env), Adv)).main() @ &m : res] -
     Pr[DDH2(KeyEx.DDH_Adv(CompEnv(Env), Adv)).main() @ &m : res]|.
 proof.
 move => pre func_eq adv_eq.
-by apply (SMCSec1 Adv Env func adv &m).
+rewrite (smc_sec1_ke_real_bridge Adv Env func adv &m) //.
+rewrite (smc_sec1_ke_ideal_bridge (KeyEx.KESim(Adv)) Env func adv &m) //.
+apply (KeyEx.ke_security Adv (CompEnv(Env)) (func ++ [2]) adv &m) => //.
+by apply exper_pre_ext1.
+qed.
+
+end section.
+
+lemma smc_security1
+        (Adv <: FUNC{MI, SMCReal, KeyEx.KEReal, KeyEx.KEIdeal,
+                     KeyEx.KESim, KeyEx.DDH_Adv, CompEnv})
+        (Env <: ENV{Adv, MI, SMCReal, KeyEx.KEReal, KeyEx.KEIdeal,
+                    KeyEx.KESim, KeyEx.DDH_Adv, CompEnv})
+        (func adv : addr) &m :
+  exper_pre func adv (fset1 adv_fw_pi) =>
+  KeyEx.DDH_Adv.func{m} = func ++ [2] => KeyEx.DDH_Adv.adv{m} = adv =>
+  `|Pr[Exper(MI(SMCReal(KeyEx.KEReal), Adv), Env).main
+         (func, adv, fset1 adv_fw_pi) @ &m : res] -
+    Pr[Exper(MI(SMCReal(KeyEx.KEIdeal), KeyEx.KESim(Adv)), Env).main
+         (func, adv, fset1 adv_fw_pi) @ &m : res]| <=
+  `|Pr[DDH1(KeyEx.DDH_Adv(CompEnv(Env), Adv)).main() @ &m : res] -
+    Pr[DDH2(KeyEx.DDH_Adv(CompEnv(Env), Adv)).main() @ &m : res]|.
+proof.
+move => pre func_eq adv_eq.
+by apply (smc_sec1 Adv Env func adv &m).
+qed.
+
+op pad_iso (x : bits, q : exp) : exp = log (gen q ^^ x).
+  
+lemma pad_isoK (x : bits) : involutive (pad_iso x).
+proof.
+rewrite /involutive /cancel /pad_iso => q.
+by rewrite gen_logK xorA xorK xor_0 log_genK.
+qed.
+
+type smc_sec2_st = {
+  smc_sec2_st_func  : addr;
+  smc_sec2_st_smcrs : smc_real_state;
+  smc_sec2_st_fws   : Fwd.fw_state;
+  smc_sec2_st_keis  : KeyEx.ke_ideal_state;
+  smc_sec2_st_smcis : smc_ideal_state;
+  smc_sec2_st_smcss : smc_sim_state
+}.
+
+pred smc_sec2_rel0 (st : smc_sec2_st) =
+  (st.`smc_sec2_st_smcrs = SMCRealStateWaitReq) /\
+  (st.`smc_sec2_st_fws   = Fwd.FwStateInit) /\
+  (st.`smc_sec2_st_keis  = KeyEx.KEIdealStateWaitReq1) /\
+  (st.`smc_sec2_st_smcis = SMCIdealStateWaitReq) /\
+  (st.`smc_sec2_st_smcss = SMCSimStateWaitReq).
+
+pred smc_sec2_rel1 (st : smc_sec2_st, pt1 pt2 : port, x : bits, q : exp) =
+  ! st.`smc_sec2_st_func <= pt1.`1 /\ ! st.`smc_sec2_st_func <= pt2.`1 /\ 
+  (st.`smc_sec2_st_smcrs = SMCRealStateWaitKE1 (pt1, pt2, x)) /\
+  (st.`smc_sec2_st_fws   = Fwd.FwStateInit) /\
+  (st.`smc_sec2_st_keis  = KeyEx.KEIdealStateWaitSim1 ((st.`smc_sec2_st_func, 1), (st.`smc_sec2_st_func, 2), q)) /\
+  (st.`smc_sec2_st_smcis = SMCIdealStateWaitSim (pt1, pt2, x)) /\
+  (st.`smc_sec2_st_smcss = SMCSimStateWaitAdv1 (st.`smc_sec2_st_func, pad_iso x q)).
+
+pred smc_sec2_rel2 (st : smc_sec2_st, pt1 pt2 : port, x : bits, q : exp) =
+  ! st.`smc_sec2_st_func <= pt1.`1 /\ ! st.`smc_sec2_st_func <= pt2.`1 /\ 
+  (st.`smc_sec2_st_smcrs = SMCRealStateWaitKE2 (pt1, pt2, x, g ^ q)) /\
+  (st.`smc_sec2_st_fws   = Fwd.FwStateInit) /\
+  (st.`smc_sec2_st_keis  = KeyEx.KEIdealStateWaitSim2 ((st.`smc_sec2_st_func, 1), (st.`smc_sec2_st_func, 2), q)) /\
+  (st.`smc_sec2_st_smcis = SMCIdealStateWaitSim (pt1, pt2, x)) /\
+  (st.`smc_sec2_st_smcss = SMCSimStateWaitAdv2 (st.`smc_sec2_st_func, pad_iso x q)).
+
+pred smc_sec2_rel3 (st : smc_sec2_st, pt1 pt2 : port, x : bits, q : exp) =
+  ! st.`smc_sec2_st_func <= pt1.`1 /\ ! st.`smc_sec2_st_func <= pt2.`1 /\ 
+  (st.`smc_sec2_st_smcrs =
+     SMCRealStateWaitFwd (pt1, pt2, x, g ^ q, g ^ q)) /\
+  (st.`smc_sec2_st_fws   =
+     Fwd.FwStateWait
+     ((st.`smc_sec2_st_func, 1), (st.`smc_sec2_st_func, 2), UnivBase (BaseBits (x ^^ g ^ q)))) /\
+  (st.`smc_sec2_st_keis  = KeyEx.KEIdealStateFinal ((st.`smc_sec2_st_func, 1), (st.`smc_sec2_st_func, 2), q)) /\
+  (st.`smc_sec2_st_smcis = SMCIdealStateWaitSim (pt1, pt2, x)) /\
+  (st.`smc_sec2_st_smcss = SMCSimStateWaitAdv3 (st.`smc_sec2_st_func, pad_iso x q)).
+
+pred smc_sec2_rel4 (st : smc_sec2_st, pt1, pt2 : port, x : bits, q : exp) =
+  (st.`smc_sec2_st_smcrs = SMCRealStateFinal (pt1, pt2, x, g ^ q, g ^ q)) /\
+  (st.`smc_sec2_st_fws   =
+     Fwd.FwStateFinal
+     ((st.`smc_sec2_st_func, 1), (st.`smc_sec2_st_func, 2), UnivBase (BaseBits (x ^^ g ^ q)))) /\
+  (st.`smc_sec2_st_keis  = KeyEx.KEIdealStateFinal ((st.`smc_sec2_st_func, 1), (st.`smc_sec2_st_func, 2), q)) /\
+  (st.`smc_sec2_st_smcis = SMCIdealStateFinal (pt1, pt2, x)) /\
+  (st.`smc_sec2_st_smcss = SMCSimStateFinal (st.`smc_sec2_st_func, pad_iso x q)).
+
+inductive smc_sec2_rel (st : smc_sec2_st) =
+    SMCSec2Rel0 of (smc_sec2_rel0 st)
+  | SMCSec2Rel1 (pt1 pt2 : port, x : bits, q : exp) of
+      (smc_sec2_rel1 st pt1 pt2 x q)
+  | SMCSec2Rel2 (pt1 pt2 : port, x : bits, q : exp) of
+      (smc_sec2_rel2 st pt1 pt2 x q)
+  | SMCSec2Rel3 (pt1 pt2 : port, x : bits, q : exp) of
+      (smc_sec2_rel3 st pt1 pt2 x q)
+  | SMCSec2Rel4 (pt1 pt2 : port, x : bits, q : exp) of
+      (smc_sec2_rel4 st pt1 pt2 x q).
+
+inductive smc_sec2_rel_1_4 (st : smc_sec2_st) =
+    SMCSec2Rel1_1_4 (pt1 pt2 : port, x : bits, q : exp) of
+      (smc_sec2_rel1 st pt1 pt2 x q)
+  | SMCSec2Rel2_1_4 (pt1 pt2 : port, x : bits, q : exp) of
+      (smc_sec2_rel2 st pt1 pt2 x q)
+  | SMCSec2Rel3_1_4 (pt1 pt2 : port, x : bits, q : exp) of
+      (smc_sec2_rel3 st pt1 pt2 x q)
+  | SMCSec2Rel4_1_4 (pt1 pt2 : port, x : bits, q : exp) of
+      (smc_sec2_rel4 st pt1 pt2 x q).
+
+inductive smc_sec2_rel_2_4 (st : smc_sec2_st) =
+    SMCSec2Rel2_2_4 (pt1 pt2 : port, x : bits, q : exp) of
+      (smc_sec2_rel2 st pt1 pt2 x q)
+  | SMCSec2Rel3_2_4 (pt1 pt2 : port, x : bits, q : exp) of
+      (smc_sec2_rel3 st pt1 pt2 x q)
+  | SMCSec2Rel4_2_4 (pt1 pt2 : port, x : bits, q : exp) of
+      (smc_sec2_rel4 st pt1 pt2 x q).
+
+inductive smc_sec2_rel_3_4 (st : smc_sec2_st) =
+    SMCSec2Rel3_3_4 (pt1 pt2 : port, x : bits, q : exp) of
+      (smc_sec2_rel3 st pt1 pt2 x q)
+  | SMCSec2Rel4_3_4 (pt1 pt2 : port, x : bits, q : exp) of
+      (smc_sec2_rel4 st pt1 pt2 x q).
+
+inductive smc_sec2_rel_4_4 (st : smc_sec2_st) =
+    SMCSec2Rel4_4_4 (pt1 pt2 : port, x : bits, q : exp) of
+      (smc_sec2_rel4 st pt1 pt2 x q).
+
+lemma smc_sec2_rel_1_4_imp_full (st : smc_sec2_st) :
+  smc_sec2_rel_1_4 st => smc_sec2_rel st.
+proof.
+case;
+  [apply SMCSec2Rel1 | apply SMCSec2Rel2 | apply SMCSec2Rel3 |
+   apply SMCSec2Rel4].
+qed.
+
+lemma smc_sec2_rel_2_4_imp_full (st : smc_sec2_st) :
+  smc_sec2_rel_2_4 st => smc_sec2_rel st.
+proof.
+case; [apply SMCSec2Rel2 | apply SMCSec2Rel3 | apply SMCSec2Rel4].
+qed.
+
+lemma smc_sec2_rel_3_4_imp_full (st : smc_sec2_st) :
+  smc_sec2_rel_3_4 st => smc_sec2_rel st.
+proof.
+case; [apply SMCSec2Rel3 | apply SMCSec2Rel4].
+qed.
+
+lemma smc_sec2_rel_4_imp_full (st : smc_sec2_st) :
+  smc_sec2_rel_4_4 st => smc_sec2_rel st.
+proof.
+case; apply SMCSec2Rel4.
 qed.
 
 section.
 
-declare module Adv : FUNC{SMCReal, KeyEx.KEIdeal, SMCIdeal, SMCSim}.
-declare module Env : ENV{Adv, SMCReal, KeyEx.KEIdeal, SMCIdeal, SMCSim}.
+declare module Adv : FUNC{MI, SMCReal, KeyEx.KEIdeal, SMCIdeal, SMCSim}.
+declare module Env : ENV{Adv, MI, SMCReal, KeyEx.KEIdeal, SMCIdeal, SMCSim}.
 
-lemma SMCSec2 (func adv : addr) &m :
+lemma MI_SMCReal_KEIdeal_Adv_SMCIdeal_SMCSim_Adv_invoke_4 :
+  equiv
+  [MI(SMCReal(KeyEx.KEIdeal), Adv).invoke ~
+   MI(SMCIdeal, SMCSim(Adv)).invoke :
+   ={m, MI.func, MI.adv, MI.in_guard} /\
+   exper_pre MI.func{1} MI.adv{1} (fset1 adv_fw_pi) /\
+   MI.in_guard{1} = fset1 adv_fw_pi /\
+   SMCReal.self{1} = MI.func{1} /\ SMCReal.adv{1} = MI.adv{1} /\
+   Fwd.Forw.self{1} = MI.func{1} ++ [1] /\
+   Fwd.Forw.adv{1} = MI.adv{1} /\
+   KeyEx.KEIdeal.self{1} = MI.func{1} ++ [2] /\
+   KeyEx.KEIdeal.adv{1} = MI.adv{1} /\
+   SMCIdeal.self{2} = MI.func{1} /\ SMCIdeal.adv{2} = MI.adv{1} /\
+   SMCSim.self{2} = MI.adv{1} /\ SMCSim.adv{2} = [] /\
+   ={glob Adv} /\
+   (exists (pt1 pt2 : port, x : bits, q : exp),
+    smc_sec2_rel4
+    {|smc_sec2_st_func = MI.func{1}; smc_sec2_st_smcrs = SMCReal.st{1};
+      smc_sec2_st_fws = Fwd.Forw.st{1}; smc_sec2_st_keis = KeyEx.KEIdeal.st{1};
+      smc_sec2_st_smcis = SMCIdeal.st{2}; smc_sec2_st_smcss = SMCSim.st{2}|}
+    pt1 pt2 x q) ==>
+   ={res, MI.func, MI.adv, MI.in_guard} /\
+   exper_pre MI.func{1} MI.adv{1} (fset1 adv_fw_pi) /\
+   MI.in_guard{1} = fset1 adv_fw_pi /\
+   SMCReal.self{1} = MI.func{1} /\ SMCReal.adv{1} = MI.adv{1} /\
+   Fwd.Forw.self{1} = MI.func{1} ++ [1] /\
+   Fwd.Forw.adv{1} = MI.adv{1} /\
+   KeyEx.KEIdeal.self{1} = MI.func{1} ++ [2] /\
+   KeyEx.KEIdeal.adv{1} = MI.adv{1} /\
+   SMCIdeal.self{2} = MI.func{1} /\ SMCIdeal.adv{2} = MI.adv{1} /\
+   SMCSim.self{2} = MI.adv{1} /\ SMCSim.adv{2} = [] /\
+   ={glob Adv} /\
+   smc_sec2_rel_4_4
+   {|smc_sec2_st_func = MI.func{1}; smc_sec2_st_smcrs = SMCReal.st{1};
+     smc_sec2_st_fws = Fwd.Forw.st{1}; smc_sec2_st_keis = KeyEx.KEIdeal.st{1};
+     smc_sec2_st_smcis = SMCIdeal.st{2}; smc_sec2_st_smcss = SMCSim.st{2}|}].
+proof.
+admit.
+qed.
+
+lemma MI_SMCReal_KEIdeal_Adv_SMCIdeal_SMCSim_Adv_invoke_3 :
+  equiv
+  [MI(SMCReal(KeyEx.KEIdeal), Adv).invoke ~
+   MI(SMCIdeal, SMCSim(Adv)).invoke :
+   ={m, MI.func, MI.adv, MI.in_guard} /\
+   exper_pre MI.func{1} MI.adv{1} (fset1 adv_fw_pi) /\
+   MI.in_guard{1} = fset1 adv_fw_pi /\
+   SMCReal.self{1} = MI.func{1} /\ SMCReal.adv{1} = MI.adv{1} /\
+   Fwd.Forw.self{1} = MI.func{1} ++ [1] /\
+   Fwd.Forw.adv{1} = MI.adv{1} /\
+   KeyEx.KEIdeal.self{1} = MI.func{1} ++ [2] /\
+   KeyEx.KEIdeal.adv{1} = MI.adv{1} /\
+   SMCIdeal.self{2} = MI.func{1} /\ SMCIdeal.adv{2} = MI.adv{1} /\
+   SMCSim.self{2} = MI.adv{1} /\ SMCSim.adv{2} = [] /\
+   ={glob Adv} /\
+   (exists (pt1 pt2 : port, x : bits, q : exp),
+    smc_sec2_rel3
+    {|smc_sec2_st_func = MI.func{1}; smc_sec2_st_smcrs = SMCReal.st{1};
+      smc_sec2_st_fws = Fwd.Forw.st{1}; smc_sec2_st_keis = KeyEx.KEIdeal.st{1};
+      smc_sec2_st_smcis = SMCIdeal.st{2}; smc_sec2_st_smcss = SMCSim.st{2}|}
+    pt1 pt2 x q) ==>
+   ={res, MI.func, MI.adv, MI.in_guard} /\
+   exper_pre MI.func{1} MI.adv{1} (fset1 adv_fw_pi) /\
+   MI.in_guard{1} = fset1 adv_fw_pi /\
+   SMCReal.self{1} = MI.func{1} /\ SMCReal.adv{1} = MI.adv{1} /\
+   Fwd.Forw.self{1} = MI.func{1} ++ [1] /\
+   Fwd.Forw.adv{1} = MI.adv{1} /\
+   KeyEx.KEIdeal.self{1} = MI.func{1} ++ [2] /\
+   KeyEx.KEIdeal.adv{1} = MI.adv{1} /\
+   SMCIdeal.self{2} = MI.func{1} /\ SMCIdeal.adv{2} = MI.adv{1} /\
+   SMCSim.self{2} = MI.adv{1} /\ SMCSim.adv{2} = [] /\
+   ={glob Adv} /\
+   smc_sec2_rel_3_4
+   {|smc_sec2_st_func = MI.func{1}; smc_sec2_st_smcrs = SMCReal.st{1};
+     smc_sec2_st_fws = Fwd.Forw.st{1}; smc_sec2_st_keis = KeyEx.KEIdeal.st{1};
+     smc_sec2_st_smcis = SMCIdeal.st{2}; smc_sec2_st_smcss = SMCSim.st{2}|}].
+proof.
+admit.
+qed.
+
+lemma MI_SMCReal_KEIdeal_Adv_SMCIdeal_SMCSim_Adv_invoke_2 :
+  equiv
+  [MI(SMCReal(KeyEx.KEIdeal), Adv).invoke ~
+   MI(SMCIdeal, SMCSim(Adv)).invoke :
+   ={m, MI.func, MI.adv, MI.in_guard} /\
+   exper_pre MI.func{1} MI.adv{1} (fset1 adv_fw_pi) /\
+   MI.in_guard{1} = fset1 adv_fw_pi /\
+   SMCReal.self{1} = MI.func{1} /\ SMCReal.adv{1} = MI.adv{1} /\
+   Fwd.Forw.self{1} = MI.func{1} ++ [1] /\
+   Fwd.Forw.adv{1} = MI.adv{1} /\
+   KeyEx.KEIdeal.self{1} = MI.func{1} ++ [2] /\
+   KeyEx.KEIdeal.adv{1} = MI.adv{1} /\
+   SMCIdeal.self{2} = MI.func{1} /\ SMCIdeal.adv{2} = MI.adv{1} /\
+   SMCSim.self{2} = MI.adv{1} /\ SMCSim.adv{2} = [] /\
+   ={glob Adv} /\
+   (exists (pt1 pt2 : port, x : bits, q : exp),
+    smc_sec2_rel2
+    {|smc_sec2_st_func = MI.func{1}; smc_sec2_st_smcrs = SMCReal.st{1};
+      smc_sec2_st_fws = Fwd.Forw.st{1}; smc_sec2_st_keis = KeyEx.KEIdeal.st{1};
+      smc_sec2_st_smcis = SMCIdeal.st{2}; smc_sec2_st_smcss = SMCSim.st{2}|}
+    pt1 pt2 x q) ==>
+   ={res, MI.func, MI.adv, MI.in_guard} /\
+   exper_pre MI.func{1} MI.adv{1} (fset1 adv_fw_pi) /\
+   MI.in_guard{1} = fset1 adv_fw_pi /\
+   SMCReal.self{1} = MI.func{1} /\ SMCReal.adv{1} = MI.adv{1} /\
+   Fwd.Forw.self{1} = MI.func{1} ++ [1] /\
+   Fwd.Forw.adv{1} = MI.adv{1} /\
+   KeyEx.KEIdeal.self{1} = MI.func{1} ++ [2] /\
+   KeyEx.KEIdeal.adv{1} = MI.adv{1} /\
+   SMCIdeal.self{2} = MI.func{1} /\ SMCIdeal.adv{2} = MI.adv{1} /\
+   SMCSim.self{2} = MI.adv{1} /\ SMCSim.adv{2} = [] /\
+   ={glob Adv} /\
+   smc_sec2_rel_2_4
+   {|smc_sec2_st_func = MI.func{1}; smc_sec2_st_smcrs = SMCReal.st{1};
+     smc_sec2_st_fws = Fwd.Forw.st{1}; smc_sec2_st_keis = KeyEx.KEIdeal.st{1};
+     smc_sec2_st_smcis = SMCIdeal.st{2}; smc_sec2_st_smcss = SMCSim.st{2}|}].
+proof.
+admit.
+qed.
+
+lemma MI_SMCReal_KEIdeal_Adv_SMCIdeal_SMCSim_Adv_invoke_1 :
+  equiv
+  [MI(SMCReal(KeyEx.KEIdeal), Adv).invoke ~
+   MI(SMCIdeal, SMCSim(Adv)).invoke :
+   ={m, MI.func, MI.adv, MI.in_guard} /\
+   exper_pre MI.func{1} MI.adv{1} (fset1 adv_fw_pi) /\
+   MI.in_guard{1} = fset1 adv_fw_pi /\
+   SMCReal.self{1} = MI.func{1} /\ SMCReal.adv{1} = MI.adv{1} /\
+   Fwd.Forw.self{1} = MI.func{1} ++ [1] /\
+   Fwd.Forw.adv{1} = MI.adv{1} /\
+   KeyEx.KEIdeal.self{1} = MI.func{1} ++ [2] /\
+   KeyEx.KEIdeal.adv{1} = MI.adv{1} /\
+   SMCIdeal.self{2} = MI.func{1} /\ SMCIdeal.adv{2} = MI.adv{1} /\
+   SMCSim.self{2} = MI.adv{1} /\ SMCSim.adv{2} = [] /\
+   ={glob Adv} /\
+   (exists (pt1 pt2 : port, x : bits, q : exp),
+    smc_sec2_rel1
+    {|smc_sec2_st_func = MI.func{1}; smc_sec2_st_smcrs = SMCReal.st{1};
+      smc_sec2_st_fws = Fwd.Forw.st{1}; smc_sec2_st_keis = KeyEx.KEIdeal.st{1};
+      smc_sec2_st_smcis = SMCIdeal.st{2}; smc_sec2_st_smcss = SMCSim.st{2}|}
+    pt1 pt2 x q) ==>
+   ={res, MI.func, MI.adv, MI.in_guard} /\
+   exper_pre MI.func{1} MI.adv{1} (fset1 adv_fw_pi) /\
+   MI.in_guard{1} = fset1 adv_fw_pi /\
+   SMCReal.self{1} = MI.func{1} /\ SMCReal.adv{1} = MI.adv{1} /\
+   Fwd.Forw.self{1} = MI.func{1} ++ [1] /\
+   Fwd.Forw.adv{1} = MI.adv{1} /\
+   KeyEx.KEIdeal.self{1} = MI.func{1} ++ [2] /\
+   KeyEx.KEIdeal.adv{1} = MI.adv{1} /\
+   SMCIdeal.self{2} = MI.func{1} /\ SMCIdeal.adv{2} = MI.adv{1} /\
+   SMCSim.self{2} = MI.adv{1} /\ SMCSim.adv{2} = [] /\
+   ={glob Adv} /\
+   smc_sec2_rel_1_4
+   {|smc_sec2_st_func = MI.func{1}; smc_sec2_st_smcrs = SMCReal.st{1};
+     smc_sec2_st_fws = Fwd.Forw.st{1}; smc_sec2_st_keis = KeyEx.KEIdeal.st{1};
+     smc_sec2_st_smcis = SMCIdeal.st{2}; smc_sec2_st_smcss = SMCSim.st{2}|}].
+proof.
+admit.
+qed.
+
+lemma MI_SMCReal_KEIdeal_Adv_SMCIdeal_SMCSim_Adv_invoke_0 :
+  equiv
+  [MI(SMCReal(KeyEx.KEIdeal), Adv).invoke ~
+   MI(SMCIdeal, SMCSim(Adv)).invoke :
+   ={m, MI.func, MI.adv, MI.in_guard} /\
+   exper_pre MI.func{1} MI.adv{1} (fset1 adv_fw_pi) /\
+   MI.in_guard{1} = fset1 adv_fw_pi /\
+   SMCReal.self{1} = MI.func{1} /\ SMCReal.adv{1} = MI.adv{1} /\
+   Fwd.Forw.self{1} = MI.func{1} ++ [1] /\
+   Fwd.Forw.adv{1} = MI.adv{1} /\
+   KeyEx.KEIdeal.self{1} = MI.func{1} ++ [2] /\
+   KeyEx.KEIdeal.adv{1} = MI.adv{1} /\
+   SMCIdeal.self{2} = MI.func{1} /\ SMCIdeal.adv{2} = MI.adv{1} /\
+   SMCSim.self{2} = MI.adv{1} /\ SMCSim.adv{2} = [] /\
+   ={glob Adv} /\
+   smc_sec2_rel0
+   {|smc_sec2_st_func = MI.func{1}; smc_sec2_st_smcrs = SMCReal.st{1};
+     smc_sec2_st_fws = Fwd.Forw.st{1}; smc_sec2_st_keis = KeyEx.KEIdeal.st{1};
+     smc_sec2_st_smcis = SMCIdeal.st{2}; smc_sec2_st_smcss = SMCSim.st{2}|} ==>
+   ={res, MI.func, MI.adv, MI.in_guard} /\
+   exper_pre MI.func{1} MI.adv{1} (fset1 adv_fw_pi) /\
+   MI.in_guard{1} = fset1 adv_fw_pi /\
+   SMCReal.self{1} = MI.func{1} /\ SMCReal.adv{1} = MI.adv{1} /\
+   Fwd.Forw.self{1} = MI.func{1} ++ [1] /\
+   Fwd.Forw.adv{1} = MI.adv{1} /\
+   KeyEx.KEIdeal.self{1} = MI.func{1} ++ [2] /\
+   KeyEx.KEIdeal.adv{1} = MI.adv{1} /\
+   SMCIdeal.self{2} = MI.func{1} /\ SMCIdeal.adv{2} = MI.adv{1} /\
+   SMCSim.self{2} = MI.adv{1} /\ SMCSim.adv{2} = [] /\
+   ={glob Adv} /\
+   smc_sec2_rel
+   {|smc_sec2_st_func = MI.func{1}; smc_sec2_st_smcrs = SMCReal.st{1};
+     smc_sec2_st_fws = Fwd.Forw.st{1}; smc_sec2_st_keis = KeyEx.KEIdeal.st{1};
+     smc_sec2_st_smcis = SMCIdeal.st{2}; smc_sec2_st_smcss = SMCSim.st{2}|}].
+proof.
+proc.
+sp 2 2.
+if => //; last first.
+auto; progress; by apply SMCSec2Rel0.
+inline MI(SMCReal(KeyEx.KEIdeal), Adv).loop
+       MI(SMCIdeal, SMCSim(Adv)).loop.
+sp 3 3.
+rcondt{1} 1; first progress. rcondt{2} 1; first progress.
+sp 2 2.
+if => //.
+inline{1} (1) SMCReal(KeyEx.KEIdeal).invoke.
+inline{2} (1) SMCIdeal.invoke.
+sp 4 4.
+if => //.
+progress; smt(inc_ext2).
+admit.
+rcondt{1} 2; first auto.
+rcondt{2} 2; first auto.
+rcondf{1} 3; first auto.
+rcondf{2} 3; first auto.
+auto; progress; by apply SMCSec2Rel0.
+inline{2} (1) SMCSim(Adv).invoke.
+sp 0 3.
+rcondt{2} 1.
+progress; auto; progress; smt().
+inline{2} (1) SMCSim(Adv).loop.
+rcondt{2} 4; progress; auto.
+sp 0 4.
+rcondf{2} 1; progress; auto; progress.
+have smc_pi_uniq := smc_pi_uniq.
+rewrite cons_uniq 3!in_cons in_nil 2!negb_or /= in smc_pi_uniq.
+smt(in_fset1).
+seq 1 1 :
+   (r0{1} = r2{2} /\ not_done{1} /\ not_done{2} /\
+   ={MI.func, MI.adv, MI.in_guard} /\
+   exper_pre MI.func{1} MI.adv{1} (fset1 adv_fw_pi) /\
+   MI.in_guard{1} = fset1 adv_fw_pi /\
+   SMCReal.self{1} = MI.func{1} /\ SMCReal.adv{1} = MI.adv{1} /\
+   Fwd.Forw.self{1} = MI.func{1} ++ [1] /\
+   Fwd.Forw.adv{1} = MI.adv{1} /\
+   KeyEx.KEIdeal.self{1} = MI.func{1} ++ [2] /\
+   KeyEx.KEIdeal.adv{1} = MI.adv{1} /\
+   SMCIdeal.self{2} = MI.func{1} /\  SMCIdeal.adv{2} = MI.adv{1} /\
+   SMCSim.self{2} = MI.adv{1} /\ SMCSim.adv{2} = [] /\
+   ={glob Adv} /\
+   smc_sec2_rel0
+   {|smc_sec2_st_func = MI.func{1}; smc_sec2_st_smcrs = SMCReal.st{1};
+     smc_sec2_st_fws = Fwd.Forw.st{1}; smc_sec2_st_keis = KeyEx.KEIdeal.st{1};
+     smc_sec2_st_smcis = SMCIdeal.st{2}; smc_sec2_st_smcss = SMCSim.st{2};|}).
+call (_ : true).
+auto.
+if => //.
+rcondf{1} 2; first auto.
+rcondf{2} 2; first auto.
+rcondt{2} 4; first auto.
+rcondf{2} 5; first auto.
+auto; progress; by apply SMCSec2Rel0.
+sp 3 2.
+rcondf{2} 1; first auto; progress; smt().
+rcondf{2} 1; first auto; progress; smt().
+rcondf{2} 1; first auto; progress; smt().
+rcondf{2} 2; first auto.
+rcondf{2} 4; first auto.
+sp 0 6.
+if => //.
+move => |> &1 &2 <- //.
+rcondf{1} 3; first auto.
+rcondf{2} 3; first auto.
+auto; progress; by apply SMCSec2Rel0.
+if => //.
+move => |> &1 &2 <- //.
+rcondf{1} 2; first auto.
+rcondf{2} 2; first auto.
+auto; progress; by apply SMCSec2Rel0.
+rcondt{1} 1; first auto. rcondt{2} 1; first auto.
+sp 2 2.
+elim* => addr10_R n10_R mod0_R pt10_R pt20_R u0_R addr10_L n10_L mod0_L
+         pt10_L pt20_L u0_L.
+rcondt{1} 1; first auto.
+rcondt{2} 1; first progress; auto => |> &hr <- //.
+inline{1} (1) SMCReal(KeyEx.KEIdeal).invoke.
+inline{2} (1) SMCIdeal.invoke.
+sp 4 4.
+conseq
+  (_ :
+   _ ==>
+   r0{1} = None /\ r0{2} = None /\
+   ={MI.func, MI.adv, MI.in_guard} /\
+   exper_pre MI.func{1} MI.adv{1} (fset1 adv_fw_pi) /\
+   MI.in_guard{1} = fset1 adv_fw_pi /\
+   SMCReal.self{1} = MI.func{1} /\
+   SMCReal.adv{1} = MI.adv{1} /\
+   Fwd.Forw.self{1} = MI.func{1} ++ [1] /\
+   Fwd.Forw.adv{1} = MI.adv{1} /\
+   KeyEx.KEIdeal.self{1} = MI.func{1} ++ [2] /\
+   KeyEx.KEIdeal.adv{1} = MI.adv{1} /\
+   SMCIdeal.self{2} = MI.func{1} /\
+   SMCIdeal.adv{2} = MI.adv{1} /\
+   SMCSim.self{2} = MI.adv{1} /\
+   SMCSim.adv{2} = [] /\
+   ={glob Adv} /\
+   smc_sec2_rel
+    {|smc_sec2_st_func = MI.func{1}; smc_sec2_st_smcrs = SMCReal.st{1};
+      smc_sec2_st_fws = Fwd.Forw.st{1}; smc_sec2_st_keis = KeyEx.KEIdeal.st{1};
+      smc_sec2_st_smcis = SMCIdeal.st{2}; smc_sec2_st_smcss = SMCSim.st{2};|}) => //.
+rcondf{2} 1.
+auto => |> &hr <-; progress; smt().
+rcondt{2} 2; first auto.
+rcondf{2} 3; first auto.
+if{1}.
+inline{1} (1) SMCReal(KeyEx.KEIdeal).loop.
+rcondt{1} 4; first auto.
+sp 3 0.
+if{1}.
+inline{1} (1) SMCReal(KeyEx.KEIdeal).parties.
+sp 2 0.
+rcondt{1} 1.
+progress; auto; progress; smt().
+rcondf{1} 1.
+progress; auto; progress.
+rewrite /is_smc_req /dec_smc_req /#.
+rcondt{1} 2; first auto.
+rcondf{1} 3; first auto.
+rcondt{1} 5.
+progress; auto; progress.
+rcondf{1} 6; first auto.
+auto; progress; by apply SMCSec2Rel0.
+if{1}.
+inline{1} (1) Fwd.Forw.invoke.
+rcondt{1} 3.
+progress; auto; smt().
+rcondf{1} 3.
+progress; auto; progress.
+rewrite /is_fw_req /dec_fw_req /#.
+rcondt{1} 4; first auto.
+rcondf{1} 5; first auto.
+rcondt{1} 7; first auto.
+rcondf{1} 8; first auto.
+auto; progress; by apply SMCSec2Rel0.
+inline{1} (1) KeyEx.KEIdeal.invoke.
+rcondf{1} 5.
+progress; auto; progress; smt().
+rcondf{1} 6; first auto.
+rcondt{1} 6; first auto.
+rcondf{1} 7; first auto.
+rcondt{1} 9; first auto.
+rcondf{1} 10; first auto.
+auto; progress; by apply SMCSec2Rel0.
+rcondt{1} 2; first auto.
+rcondf{1} 3; first auto.
+auto; progress; by apply SMCSec2Rel0.
+qed.
+
+lemma MI_SMCReal_KEIdeal_Adv_SMCIdeal_SMCSim_Adv_invoke :
+  equiv
+  [MI(SMCReal(KeyEx.KEIdeal), Adv).invoke ~
+   MI(SMCIdeal, SMCSim(Adv)).invoke :
+   ={m, MI.func, MI.adv, MI.in_guard} /\
+   exper_pre MI.func{1} MI.adv{1} (fset1 adv_fw_pi) /\
+   MI.in_guard{1} = fset1 adv_fw_pi /\
+   SMCReal.self{1} = MI.func{1} /\ SMCReal.adv{1} = MI.adv{1} /\
+   Fwd.Forw.self{1} = MI.func{1} ++ [1] /\
+   Fwd.Forw.adv{1} = MI.adv{1} /\
+   KeyEx.KEIdeal.self{1} = MI.func{1} ++ [2] /\
+   KeyEx.KEIdeal.adv{1} = MI.adv{1} /\
+   SMCIdeal.self{2} = MI.func{1} /\ SMCIdeal.adv{2} = MI.adv{1} /\
+   SMCSim.self{2} = MI.adv{1} /\ SMCSim.adv{2} = [] /\
+   ={glob Adv} /\
+   smc_sec2_rel
+   {|smc_sec2_st_func = MI.func{1}; smc_sec2_st_smcrs = SMCReal.st{1};
+     smc_sec2_st_fws = Fwd.Forw.st{1}; smc_sec2_st_keis = KeyEx.KEIdeal.st{1};
+     smc_sec2_st_smcis = SMCIdeal.st{2}; smc_sec2_st_smcss = SMCSim.st{2}|} ==>
+   ={res, MI.func, MI.adv, MI.in_guard} /\
+   exper_pre MI.func{1} MI.adv{1} (fset1 adv_fw_pi) /\
+   MI.in_guard{1} = fset1 adv_fw_pi /\
+   SMCReal.self{1} = MI.func{1} /\ SMCReal.adv{1} = MI.adv{1} /\
+   Fwd.Forw.self{1} = MI.func{1} ++ [1] /\
+   Fwd.Forw.adv{1} = MI.adv{1} /\
+   KeyEx.KEIdeal.self{1} = MI.func{1} ++ [2] /\
+   KeyEx.KEIdeal.adv{1} = MI.adv{1} /\
+   SMCIdeal.self{2} = MI.func{1} /\ SMCIdeal.adv{2} = MI.adv{1} /\
+   SMCSim.self{2} = MI.adv{1} /\ SMCSim.adv{2} = [] /\
+   ={glob Adv} /\
+   smc_sec2_rel
+   {|smc_sec2_st_func = MI.func{1}; smc_sec2_st_smcrs = SMCReal.st{1};
+     smc_sec2_st_fws = Fwd.Forw.st{1}; smc_sec2_st_keis = KeyEx.KEIdeal.st{1};
+     smc_sec2_st_smcis = SMCIdeal.st{2}; smc_sec2_st_smcss = SMCSim.st{2}|}].
+proof.
+proc*.
+case
+  (smc_sec2_rel0
+   {|smc_sec2_st_func = MI.func{1}; smc_sec2_st_smcrs = SMCReal.st{1};
+     smc_sec2_st_fws = Fwd.Forw.st{1}; smc_sec2_st_keis = KeyEx.KEIdeal.st{1};
+     smc_sec2_st_smcis = SMCIdeal.st{2}; smc_sec2_st_smcss = SMCSim.st{2};|}).
+call MI_SMCReal_KEIdeal_Adv_SMCIdeal_SMCSim_Adv_invoke_0.
+auto.
+case
+  (exists (pt1 pt2 : port, x : bits, q : exp),
+   smc_sec2_rel1
+   {|smc_sec2_st_func = MI.func{1}; smc_sec2_st_smcrs = SMCReal.st{1};
+     smc_sec2_st_fws = Fwd.Forw.st{1}; smc_sec2_st_keis = KeyEx.KEIdeal.st{1};
+     smc_sec2_st_smcis = SMCIdeal.st{2}; smc_sec2_st_smcss = SMCSim.st{2};|}
+   pt1 pt2 x q).
+call MI_SMCReal_KEIdeal_Adv_SMCIdeal_SMCSim_Adv_invoke_1.
+auto; progress.
+by exists pt1 pt2 x q.
+by apply smc_sec2_rel_1_4_imp_full.
+case
+  (exists (pt1 pt2 : port, x : bits, q : exp),
+   smc_sec2_rel2
+   {|smc_sec2_st_func = MI.func{1}; smc_sec2_st_smcrs = SMCReal.st{1};
+     smc_sec2_st_fws = Fwd.Forw.st{1}; smc_sec2_st_keis = KeyEx.KEIdeal.st{1};
+     smc_sec2_st_smcis = SMCIdeal.st{2}; smc_sec2_st_smcss = SMCSim.st{2};|}
+   pt1 pt2 x q).
+call MI_SMCReal_KEIdeal_Adv_SMCIdeal_SMCSim_Adv_invoke_2.
+auto; progress.
+by exists pt1 pt2 x q.
+by apply smc_sec2_rel_2_4_imp_full.
+case
+  (exists (pt1 pt2 : port, x : bits, q : exp),
+   smc_sec2_rel3
+   {|smc_sec2_st_func = MI.func{1}; smc_sec2_st_smcrs = SMCReal.st{1};
+     smc_sec2_st_fws = Fwd.Forw.st{1}; smc_sec2_st_keis = KeyEx.KEIdeal.st{1};
+     smc_sec2_st_smcis = SMCIdeal.st{2}; smc_sec2_st_smcss = SMCSim.st{2};|}
+   pt1 pt2 x q).
+call MI_SMCReal_KEIdeal_Adv_SMCIdeal_SMCSim_Adv_invoke_3.
+auto; progress.
+by exists pt1 pt2 x q.
+by apply smc_sec2_rel_3_4_imp_full.
+case
+  (exists (pt1 pt2 : port, x : bits, q : exp),
+   smc_sec2_rel4
+   {|smc_sec2_st_func = MI.func{1}; smc_sec2_st_smcrs = SMCReal.st{1};
+     smc_sec2_st_fws = Fwd.Forw.st{1}; smc_sec2_st_keis = KeyEx.KEIdeal.st{1};
+     smc_sec2_st_smcis = SMCIdeal.st{2}; smc_sec2_st_smcss = SMCSim.st{2};|}
+   pt1 pt2 x q).
+call MI_SMCReal_KEIdeal_Adv_SMCIdeal_SMCSim_Adv_invoke_4.
+auto; progress.
+by exists pt1 pt2 x q.
+by apply smc_sec2_rel_4_imp_full.
+exfalso => &1 &2 [# _ _ _ _ _ _ _ _ _ _ _ _ _ _ _ _ _].
+case => //.
+move => pt1 pt2 x q true1 _ false1.
+have true1_ex // : 
+  exists (pt1 pt2 : port, x : bits, q : exp),
+  smc_sec2_rel1
+   {|smc_sec2_st_func = MI.func{1}; smc_sec2_st_smcrs = SMCReal.st{1};
+     smc_sec2_st_fws = Fwd.Forw.st{1}; smc_sec2_st_keis = KeyEx.KEIdeal.st{1};
+     smc_sec2_st_smcis = SMCIdeal.st{2}; smc_sec2_st_smcss = SMCSim.st{2};|}
+  pt1 pt2 x q.
+  by exists pt1 pt2 x q.
+move => pt1 pt2 x q true2 _ _.
+have true2_ex // : 
+  exists (pt1 pt2 : port, x : bits, q : exp),
+  smc_sec2_rel2
+   {|smc_sec2_st_func = MI.func{1}; smc_sec2_st_smcrs = SMCReal.st{1};
+     smc_sec2_st_fws = Fwd.Forw.st{1}; smc_sec2_st_keis = KeyEx.KEIdeal.st{1};
+     smc_sec2_st_smcis = SMCIdeal.st{2}; smc_sec2_st_smcss = SMCSim.st{2};|}
+  pt1 pt2 x q.
+  by exists pt1 pt2 x q.
+move => pt1 pt2 x q true3 _ _ _.
+have true3_ex // : 
+  exists (pt1 pt2 : port, x : bits, q : exp),
+  smc_sec2_rel3
+   {|smc_sec2_st_func = MI.func{1}; smc_sec2_st_smcrs = SMCReal.st{1};
+     smc_sec2_st_fws = Fwd.Forw.st{1}; smc_sec2_st_keis = KeyEx.KEIdeal.st{1};
+     smc_sec2_st_smcis = SMCIdeal.st{2}; smc_sec2_st_smcss = SMCSim.st{2};|}
+  pt1 pt2 x q.
+  by exists pt1 pt2 x q.
+move => pt1 pt2 x q true4 _ _ _.
+have true4_ex // : 
+  exists (pt1 pt2 : port, x : bits, q : exp),
+  smc_sec2_rel4
+   {|smc_sec2_st_func = MI.func{1}; smc_sec2_st_smcrs = SMCReal.st{1};
+     smc_sec2_st_fws = Fwd.Forw.st{1}; smc_sec2_st_keis = KeyEx.KEIdeal.st{1};
+     smc_sec2_st_smcis = SMCIdeal.st{2}; smc_sec2_st_smcss = SMCSim.st{2};|}
+  pt1 pt2 x q.
+  by exists pt1 pt2 x q.
+qed.
+
+lemma smc_sec2 (func adv : addr) &m :
   exper_pre func adv (fset1 adv_fw_pi) =>
-  Pr[Exper(MakeInter(SMCReal(KeyEx.KEIdeal), Adv), Env).main
+  Pr[Exper(MI(SMCReal(KeyEx.KEIdeal), Adv), Env).main
        (func, adv, fset1 adv_fw_pi) @ &m : res] =
-  Pr[Exper(MakeInter(SMCIdeal, SMCSim(Adv)), Env).main
+  Pr[Exper(MI(SMCIdeal, SMCSim(Adv)), Env).main
        (func, adv, fset1 adv_fw_pi) @ &m : res].
 proof.
-move => pre.
-byequiv => //.
-proc.
-admit.
+move => pre; byequiv => //; proc.
+seq 1 1 :
+  (={func, adv, in_guard, MI.func, MI.adv, MI.in_guard} /\
+   exper_pre func{1} adv{1} (fset1 adv_fw_pi) /\
+   MI.func{1} = func{1} /\ MI.adv{1} = adv{1} /\
+   MI.in_guard{1} = fset1 adv_fw_pi /\
+   SMCReal.self{1} = func{1} /\ SMCReal.adv{1} = adv{1} /\
+   SMCReal.st{1} = SMCRealStateWaitReq /\
+   Fwd.Forw.self{1} = func{1} ++ [1] /\ Fwd.Forw.adv{1} = adv{1} /\
+   Fwd.Forw.st{1} = Fwd.FwStateInit /\
+   KeyEx.KEIdeal.self{1} = func{1} ++ [2] /\ KeyEx.KEIdeal.adv{1} = adv{1} /\
+   KeyEx.KEIdeal.st{1} = KeyEx.KEIdealStateWaitReq1 /\
+   SMCIdeal.self{2} = func{1} /\ SMCIdeal.adv{2} = adv{1} /\
+   SMCIdeal.st{2} = SMCIdealStateWaitReq /\
+   SMCSim.self{2} = adv{1} /\ SMCSim.adv{2} = [] /\
+   SMCSim.st{2} = SMCSimStateWaitReq /\
+   ={glob Adv}).
+inline*.
+swap{2} 16 1; call (_ : true).
+auto.
+auto.
+call
+  (_ : 
+   ={func, adv, in_guard, MI.func, MI.adv, MI.in_guard} /\
+   exper_pre func{1} adv{1} (fset1 adv_fw_pi) /\
+   MI.func{1} = func{1} /\ MI.adv{1} = adv{1} /\
+   MI.in_guard{1} = fset1 adv_fw_pi /\
+   SMCReal.self{1} = func{1} /\ SMCReal.adv{1} = adv{1} /\
+   Fwd.Forw.self{1} = func{1} ++ [1] /\ Fwd.Forw.adv{1} = adv{1} /\
+   KeyEx.KEIdeal.self{1} = func{1} ++ [2] /\ KeyEx.KEIdeal.adv{1} = adv{1} /\
+   SMCIdeal.self{2} = func{1} /\ SMCIdeal.adv{2} = adv{1} /\
+   SMCSim.self{2} = adv{1} /\ SMCSim.adv{2} = [] /\
+   ={glob Adv} /\
+   smc_sec2_rel
+   {|smc_sec2_st_func = func{1}; smc_sec2_st_smcrs = SMCReal.st{1};
+     smc_sec2_st_fws = Fwd.Forw.st{1}; smc_sec2_st_keis = KeyEx.KEIdeal.st{1};
+     smc_sec2_st_smcis = SMCIdeal.st{2}; smc_sec2_st_smcss = SMCSim.st{2}|} ==>
+   ={res}).
+proc
+  (={MI.func, MI.adv, MI.in_guard} /\
+   exper_pre func{1} adv{1} (fset1 adv_fw_pi) /\
+   MI.func{1} = func{1} /\ MI.adv{1} = adv{1} /\
+   MI.in_guard{1} = fset1 adv_fw_pi /\
+   SMCReal.self{1} = func{1} /\ SMCReal.adv{1} = adv{1} /\
+   Fwd.Forw.self{1} = func{1} ++ [1] /\ Fwd.Forw.adv{1} = adv{1} /\
+   KeyEx.KEIdeal.self{1} = func{1} ++ [2] /\ KeyEx.KEIdeal.adv{1} = adv{1} /\
+   SMCIdeal.self{2} = func{1} /\ SMCIdeal.adv{2} = adv{1} /\
+   SMCSim.self{2} = adv{1} /\ SMCSim.adv{2} = [] /\
+   ={glob Adv} /\
+   smc_sec2_rel
+   {|smc_sec2_st_func = func{1}; smc_sec2_st_smcrs = SMCReal.st{1};
+     smc_sec2_st_fws = Fwd.Forw.st{1}; smc_sec2_st_keis = KeyEx.KEIdeal.st{1};
+     smc_sec2_st_smcis = SMCIdeal.st{2}; smc_sec2_st_smcss = SMCSim.st{2}|}) => //.
+by conseq MI_SMCReal_KEIdeal_Adv_SMCIdeal_SMCSim_Adv_invoke.
+auto; progress; by apply SMCSec2Rel0.
 qed.
 
 end section.
 
-lemma SMCSecurity2
-        (Adv <: FUNC{SMCReal, SMCIdeal, SMCSim, KeyEx.KEIdeal})
-        (Env <: ENV{Adv, SMCReal, SMCIdeal, SMCSim, KeyEx.KEIdeal})
+lemma smc_security2
+        (Adv <: FUNC{MI, SMCReal, SMCIdeal, SMCSim, KeyEx.KEIdeal})
+        (Env <: ENV{Adv, MI, SMCReal, SMCIdeal, SMCSim, KeyEx.KEIdeal})
         (func adv : addr) &m :
   exper_pre func adv (fset1 adv_fw_pi) =>
-  Pr[Exper(MakeInter(SMCReal(KeyEx.KEIdeal), Adv), Env).main
+  Pr[Exper(MI(SMCReal(KeyEx.KEIdeal), Adv), Env).main
        (func, adv, fset1 adv_fw_pi) @ &m : res] =
-  Pr[Exper(MakeInter(SMCIdeal, SMCSim(Adv)), Env).main
+  Pr[Exper(MI(SMCIdeal, SMCSim(Adv)), Env).main
        (func, adv, fset1 adv_fw_pi) @ &m : res].
 proof.
 move => pre.
-by apply (SMCSec2 Adv Env func adv &m).
+by apply (smc_sec2 Adv Env func adv &m).
 qed.
 
-lemma SMCSecurity
-        (Adv <: FUNC{SMCReal, SMCIdeal, SMCSim, KeyEx.KEReal, KeyEx.KEIdeal,
-                     KeyEx.KESim, KeyEx.DDH_Adv})
-        (Env <: ENV{Adv, SMCReal, SMCIdeal, SMCSim, KeyEx.KEReal, KeyEx.KEIdeal,
-                    KeyEx.KESim, KeyEx.DDH_Adv})
+lemma smc_security
+        (Adv <: FUNC{MI, SMCReal, SMCIdeal, SMCSim, KeyEx.KEReal,
+                     KeyEx.KEIdeal, KeyEx.KESim, KeyEx.DDH_Adv, CompEnv})
+        (Env <: ENV{Adv, MI, SMCReal, SMCIdeal, SMCSim, KeyEx.KEReal,
+                    KeyEx.KEIdeal, KeyEx.KESim, KeyEx.DDH_Adv, CompEnv})
         (func adv : addr) &m :
   exper_pre func adv (fset1 adv_fw_pi) =>
-  KeyEx.DDH_Adv.func{m} = func => KeyEx.DDH_Adv.adv{m} = adv =>
-  `|Pr[Exper(MakeInter(SMCReal(KeyEx.KEReal), Adv), Env).main
+  KeyEx.DDH_Adv.func{m} = func ++ [2] => KeyEx.DDH_Adv.adv{m} = adv =>
+  `|Pr[Exper(MI(SMCReal(KeyEx.KEReal), Adv), Env).main
          (func, adv, fset1 adv_fw_pi) @ &m : res] -
-    Pr[Exper(MakeInter(SMCIdeal, SMCSim(KeyEx.KESim(Adv))), Env).main
+    Pr[Exper(MI(SMCIdeal, SMCSim(KeyEx.KESim(Adv))), Env).main
          (func, adv, fset1 adv_fw_pi) @ &m : res]| <=
   `|Pr[DDH1(KeyEx.DDH_Adv(CompEnv(Env), Adv)).main() @ &m : res] -
     Pr[DDH2(KeyEx.DDH_Adv(CompEnv(Env), Adv)).main() @ &m : res]|.
 proof.
 move => pre func_eq adv_eq.
-by rewrite -(SMCSecurity2 (KeyEx.KESim(Adv)) Env func adv &m) //
-           (SMCSecurity1 Adv Env func adv &m).
+by rewrite -(smc_security2 (KeyEx.KESim(Adv)) Env func adv &m) //
+           (smc_security1 Adv Env func adv &m).
 qed.
+
+end SMC.
